security proof done - several seemingly trivial admits.

theories/examples/authentikit_susp_security.v
@@ -4,7 +4,7 @@ From auth.heap_lang Require Import gen_weakestpre typedproph.
 From auth.heap_lang.lib Require Import list map.
 From auth.examples Require Export authentikit_susp authentikit_base_susp_security.
 From iris.base_logic.lib Require Export na_invariants.
-From iris.algebra Require Import auth agree numbers.
+From iris.algebra Require Import auth agree numbers csum excl.
 
 (* Class tableG (Σ: gFunctors) := {
   tableG_na_invG :: na_invG Σ;
@@ -16,8 +16,8 @@ Definition table_inv `{!invGS_gen hlc Σ} `{!tableG Σ} (N : namespace) (P : iPr
 Definition table_tok `{!invGS_gen hlc Σ} `{!tableG Σ} (E : coPset) :=
   na_own tableG_name E. *)
 
-Definition idcntrUR := authUR nat.
-Class idcntrG Σ := IdcntrG { idcntr_inG :> inG Σ idcntrUR; idcntrG_name : gname }.
+(* Definition idcntrUR := authUR nat.
+Class idcntrG Σ := IdcntrG { idcntr_inG :> inG Σ idcntrUR; idcntrG_name : gname }. *)
 
 (* Definition msizeUR := authUR natUR.
 Class msizeG Σ := MsizeG { msize_inG :> inG Σ msizeUR; msizeG_name : gname }.
@@ -33,14 +33,14 @@ Proof.
   by iFrame.
 Admitted. *)
 
-Lemma idcntr_alloc `{inG Σ idcntrUR} :
+(* Lemma idcntr_alloc `{inG Σ idcntrUR} :
   ⊢ |==> ∃ _ : idcntrG Σ, (own idcntrG_name (●{DfracOwn (1/2)} 0) ∗ own idcntrG_name (●{DfracOwn (1/2)} 0))%I.
 Proof.
   iMod (own_alloc (● 0 ⋅ ◯ 0)) as (γ) "[Hauth _]"; [admit|].
   set (H1 := IdcntrG _ _ γ).
   iExists _.
   by iDestruct "Hauth" as "[$ $]".
-Admitted.
+Admitted. *)
 
 (* Lemma state_alloc `{inG Σ stateUR} :
   ⊢ |==> ∃ _ : stateG Σ, (own stateG_name (● (∅, ∅)))%I.
@@ -48,9 +48,22 @@ Proof.
   iMod (own_alloc ((● (∅, ∅)) : stateUR)) as (γ) "Hst"; [admit|].
   by iExists (StateG _ _ γ).
 Admitted. *)
+
+Definition poisonOSR := authUR (optionUR (optionUR (agree unitUR))).
+Class poisonOSG Σ := PoisonOSG { poisonOS_inG :> inG Σ poisonOSR; poisonOSG_name : gname }.
+
+Lemma pos_alloc `{inG Σ poisonOSR} :
+  ⊢ |==> ∃ _ : poisonOSG Σ, 
+      (own poisonOSG_name (●{DfracOwn (1/2)} None)) ∗ 
+      (own poisonOSG_name (●{DfracOwn (1/2)} None))%I.
+Proof.
+  iMod (own_alloc (● None)) as (γ) "[Hauth1 Hauth2]"; [admit|].
+  set (H1 := PoisonOSG _ _ γ).
+  iExists _. by iFrame.
+Admitted.
   
 Section proof.
-  Context `{!idcntrG Σ, !authG Σ, !seqG Σ}.
+  Context `{!authG Σ, !seqG Σ, !poisonOSG Σ}.
 
   Definition authBaseN : namespace := nroot .@ "susp_ver".
   Definition gmapN : namespace := authBaseN .@ "gmap".
@@ -63,7 +76,20 @@ Section proof.
   Definition msize_frag (n : nat) : iProp Σ :=
     own msizeG_name (●{DfracOwn (1/2)} n). *)
 
-  Definition idcntr_frag (n : nat) := own idcntrG_name (●{DfracOwn (1/2)} n).
+  (* Definition idcntr_frag (n : nat) := own idcntrG_name (●{DfracOwn (1/2)} n). *)
+
+  Definition pos_car := optionUR (optionUR (agree unitUR)).
+
+  Definition pos (o : pos_car) := own poisonOSG_name (●{DfracOwn (1/2)} o).
+  Definition good_pos := pos None.
+  Definition bad_pos := pos (Some None).
+  Definition done_pos := pos (Some (Some (to_agree ()))).
+  Definition valid_pos o : iProp Σ := pos o ∧ ⌜o = None ∨ o = Some None⌝.
+
+  Definition pos_frag (o : pos_car) := own poisonOSG_name (◯ o).
+  Definition good_pos_frag := pos_frag None.
+  Definition bad_pos_frag := pos_frag (Some None).
+  Definition done_pos_frag := pos_frag (Some (Some (to_agree ()))).
 
   Local Notation s_is_ser_proph := (s_is_ser_proph authBaseN).
   Local Notation ser_spec_un := (ser_spec_un authBaseN).
@@ -73,6 +99,26 @@ Section proof.
 
   Local Notation lrel_evidence := (lrel_evidence authBaseN).
   Local Notation lrel_auth := (lrel_auth authBaseN).
+
+  (* Lemma get_frag (o : pos_car) :
+    pos o -∗ pos o ∗ pos_frag o.
+  Proof. Admitted. *)
+
+  Lemma pos_agree (o o' : pos_car) :
+    pos o -∗ pos o' -∗ ⌜o' = o⌝ ∗ pos o ∗ pos o'.
+  Proof. Admitted.
+
+  Lemma pos_auth_frag_valid (o o' : pos_car) :
+    pos o -∗ pos_frag o' -∗ ⌜o' ≼ o⌝ ∗ pos o ∗ pos_frag o'.
+  Proof. Admitted.
+
+  Lemma pos_update1 :
+    good_pos -∗ good_pos ==∗ bad_pos ∗ bad_pos ∗ bad_pos_frag.
+  Proof. Admitted.
+
+  Lemma pos_update2 :
+    bad_pos -∗ bad_pos ==∗ done_pos ∗ done_pos ∗ done_pos_frag.
+  Proof. Admitted.
 
 
   (* Definition proph_type : Type := nat * option unit.
@@ -168,27 +214,13 @@ Section proof.
     destruct v; simpl; [destruct u|]; f_equal.
   Qed. *)
 
-  Definition finish_spec1 (finish : val) (x a aᵥ aᵢ ser : val) (A : lrel_bi Σ) : iProp Σ :=
-    ∀ (s s' : string) (E: coPset) (t t' : evi_type),
-      ⌜↑authSet authBaseN ⊆ E⌝ -∗
-      {{{ seq_tok E ∗ ⌜a = InjLV #(hash s)⌝ ∗ hashed s ∗ ser_spec_3 ser t ∗ 
-          s_is_ser_proph t x s' ∗ s_is_ser'' t' aᵥ s ∗ lrel_bi_bin A aᵥ aᵢ }}}
-            (* ser_spec_3 ser t  ∗
-            val_eq_rel authBaseN (lrel_bi_bin A) ∗ val_eq_rel_un authBaseN (lrel_bi_un A) ∗ *)
-            (* s_is_ser'' t' aᵥ s ∗ ⌜a = InjLV #(hash s)⌝ }}} *)
-        finish #()
-        {{{ (o : option val), RET $o;
-        (* We might prophesy that the filled-in value is the correct one,
-           But it is still possible that the value isn't actually filled. *)
-            seq_tok E ∗ if o is None then True else ⌜s = s'⌝ }}}.
+  (* map size is always > 1, if poison value then finish returns none *)
 
-  Definition finish_spec2 (finish : val) (x a aᵥ aᵢ ser : val) (A : lrel_bi Σ) : iProp Σ :=
-    ∀ (s s' h : string) (E: coPset) (t t' : evi_type) (susp : loc),
-      ⌜↑authSet authBaseN ⊆ E ∧ ↑tableN ⊆ E⌝ -∗
-      {{{ seq_tok E ∗ ⌜a = InjRV #susp⌝ ∗ ser_spec_3 ser t ∗ hashed s ∗
-          seq_inv (authN authBaseN susp) (auth_inv h susp) ∗
-          s_is_ser_proph t x s' ∗ s_is_ser'' t' aᵥ s ∗ lrel_bi_bin A aᵥ aᵢ ∗
-          ⌜h = some_ser_str (string_ser_str (hash s))⌝ }}}
+  Definition finish_spec1 (finish : val) (x a ser : val) : iProp Σ :=
+    ∀ (s s' : string) (E: coPset) (t : evi_type),
+      ⌜↑authSet authBaseN ⊆ E⌝ -∗
+      {{{ seq_tok E ∗ s_is_ser_proph t x s' ∗ ser_spec_3 ser t ∗
+          ⌜a = InjLV #s⌝ }}}
             (* ser_spec_3 ser t  ∗
             val_eq_rel authBaseN (lrel_bi_bin A) ∗ val_eq_rel_un authBaseN (lrel_bi_un A) ∗ *)
             (* s_is_ser'' t' aᵥ s ∗ ⌜a = InjLV #(hash s)⌝ }}} *)
@@ -196,23 +228,93 @@ Section proof.
         {{{ (o : option val), RET $o;
         (* We might prophesy that the filled-in value is the correct one,
            But it is still possible that the value isn't actually filled. *)
-            seq_tok E ∗ if o is None then True else ⌜s = s'⌝ }}}.
+            seq_tok E (* ∗ if o is None then True else A x aᵢ *) }}}.
+
+  (* Definition finish_spec1_dc (finish : val) (x a ser : val) (A : lrel_un Σ) : iProp Σ :=
+    ∀ (s s' : string) (E: coPset) (t : evi_type),
+      ⌜↑authSet authBaseN ⊆ E⌝ -∗
+      {{{ seq_tok E ∗ s_is_ser_proph t x s' ∗ ser_spec_3 ser t ∗
+          ⌜a = InjLV #s⌝ }}}
+            (* ser_spec_3 ser t  ∗
+            val_eq_rel authBaseN (lrel_bi_bin A) ∗ val_eq_rel_un authBaseN (lrel_bi_un A) ∗ *)
+            (* s_is_ser'' t' aᵥ s ∗ ⌜a = InjLV #(hash s)⌝ }}} *)
+        finish #()
+        {{{ (o : option val), RET $o;
+        (* We might prophesy that the filled-in value is the correct one,
+           But it is still possible that the value isn't actually filled. *)
+            seq_tok E ∗ if o is None then True else A x aᵢ }}}. *)
+
+  Definition finish_spec1_bad (finish : val) (x a ser : val) : iProp Σ :=
+    ∀ (s s' : string) (E: coPset) (t : evi_type),
+      ⌜↑authSet authBaseN ⊆ E⌝ -∗
+      {{{ seq_tok E ∗ s_is_ser_proph t x s' ∗ ser_spec_3 ser t ∗
+          hashed s ∗ ⌜a = InjLV #(hash s)⌝ ∗ ⌜s ≠ s'⌝ }}}
+            (* ser_spec_3 ser t  ∗
+            val_eq_rel authBaseN (lrel_bi_bin A) ∗ val_eq_rel_un authBaseN (lrel_bi_un A) ∗ *)
+            (* s_is_ser'' t' aᵥ s ∗ ⌜a = InjLV #(hash s)⌝ }}} *)
+        finish #()
+        {{{ (o : option val), RET $o; seq_tok E ∗ ⌜o = None⌝ }}}.
+
+  Definition finish_spec2 (finish : val) (x a ser : val) : iProp Σ :=
+    ∀ (s' s'' : string) (E: coPset) (t : evi_type) (susp : loc) (o' : pos_car),
+      ⌜↑authSet authBaseN ⊆ E ∧ ↑tableN ⊆ E⌝ -∗
+      {{{ seq_tok E ∗ s_is_ser_proph t x s' ∗ ser_spec_3 ser t ∗ valid_pos o' ∗ 
+          ⌜a = InjRV #susp⌝ ∗ seq_inv (authN authBaseN susp) (auth_inv s'' susp) }}}
+            (* ser_spec_3 ser t  ∗
+            val_eq_rel authBaseN (lrel_bi_bin A) ∗ val_eq_rel_un authBaseN (lrel_bi_un A) ∗ *)
+            (* s_is_ser'' t' aᵥ s ∗ ⌜a = InjLV #(hash s)⌝ }}} *)
+        finish #()
+        {{{ (o : option val), RET $o;
+        (* We might prophesy that the filled-in value is the correct one,
+           But it is still possible that the value isn't actually filled. *)
+            seq_tok E ∗ (if o is Some _ then pos o' else True) }}}.
+
+  Definition finish_spec2_bad (finish : val) (x a ser : val) : iProp Σ :=
+    ∀ (s s' s'' : string) (E: coPset) (t : evi_type) (susp : loc),
+      ⌜↑authSet authBaseN ⊆ E⌝ -∗
+      {{{ seq_tok E ∗ s_is_ser_proph t x s' ∗ ser_spec_3 ser t ∗
+          ⌜a = InjRV #susp⌝ ∗ ⌜s'' = some_ser_str (string_ser_str (hash s))⌝ ∗ 
+          hashed s ∗ seq_inv (authN authBaseN susp) (auth_inv s'' susp) ∗ ⌜s ≠ s'⌝ }}}
+            (* ser_spec_3 ser t  ∗
+            val_eq_rel authBaseN (lrel_bi_bin A) ∗ val_eq_rel_un authBaseN (lrel_bi_un A) ∗ *)
+            (* s_is_ser'' t' aᵥ s ∗ ⌜a = InjLV #(hash s)⌝ }}} *)
+        finish #()
+        {{{ (o : option val), RET $o; seq_tok E ∗ ⌜o = None⌝ }}}.
+
+  Definition good_finish_specs (m : gmap val val) finish x a ser : iProp Σ :=
+    ((∃ (s : string), ⌜a = InjLV #s⌝ ∗ finish_spec1 finish x a ser) ∨ 
+      (∃ s'' (susp : loc), ⌜a = InjRV #susp⌝ ∗
+        seq_inv (authN authBaseN susp) (auth_inv s'' susp) ∗
+        finish_spec2 finish x a ser)).
+
+  Definition bad_finish_specs (m : gmap val val) finish x a ser s s' : iProp Σ :=
+    ((⌜a = InjLV #(hash s)⌝ ∗ hashed s ∗ 
+        (finish_spec1_bad finish x a ser ∧ ⌜s ≠ s'⌝)) ∨ 
+      (∃ s'' (susp : loc), ⌜a = InjRV #susp⌝ ∗ hashed s ∗
+        ⌜s'' = some_ser_str (string_ser_str (hash s))⌝ ∗ 
+        seq_inv (authN authBaseN susp) (auth_inv s'' susp) ∗
+          (finish_spec2_bad finish x a ser ∧ ⌜s ≠ s'⌝))).
 
   Definition susp_big_sep (m : gmap val val) : iProp Σ :=
     [∗ map] k ↦ v ∈ m,
-      ∃ (ctr : nat) (finish x a aᵥ aᵢ ser : val) (t : evi_type) (A : lrel_bi Σ) (s : string),
+      ∃ (ctr : nat) (finish x a ser : val) (t : evi_type) (s' : string),
         (⌜ctr > 0 ∧ v = (#ctr, finish)%V⌝ ∗ 
-            lrel_bi_un A x ∗ ser_spec_3 ser t ∗
-            ((⌜a = InjLV #(hash s)⌝ ∗ hashed s ∗ finish_spec1 finish x a aᵥ aᵢ ser A) ∨ 
-              (∃ (susp : loc), ⌜a = InjRV #susp⌝ ∗ finish_spec2 finish x a aᵥ aᵢ ser A ∗
-                seq_inv (authN authBaseN susp) (auth_inv s susp)))).
-           (* ∨ (∃ (susp : loc), ⌜a = InjRV #susp⌝ ∗ susp↦□ InjRV #h ∗
-                                                finish_spec2 finish x a aᵥ aᵢ ser A))). *)
+            s_is_ser_proph t x s' ∗ ser_spec_3 ser t ∗
+            (good_finish_specs m finish x a ser ∨
+              (∃ s, bad_pos_frag ∗ bad_finish_specs m finish x a ser s s'))).
+
+  Definition susp_bad_ge1 (m : gmap val val) : iProp Σ :=
+    good_pos ∨ done_pos ∨
+      (bad_pos ∗ ⌜map.map_length m > 0⌝).
+        (* (∃ (k v : val) (ctr : nat) finish x a ser t s s', 
+          ⌜map_Exists (λ k' v', v = v' ∧ k = k') m⌝ ∗
+          ⌜ctr > 0 ∧ v = (#ctr, finish)%V⌝ ∗ 
+            s_is_ser_proph t x s' ∗ ser_spec_3 ser t ∗
+            bad_finish_specs m finish x a ser s s')). *)
       
   Definition is_susp_table (l : loc) : iProp Σ :=
     ∃ (d : val) (m : gmap val val),
-      l ↦ d ∗ ⌜is_map d m⌝ ∗ susp_big_sep m.
-        (* idcntr_frag c ∗ (∀ (id : nat), ⌜id ≥ c → m !! #id = None⌝) *)
+      l ↦ d ∗ ⌜is_map d m⌝ ∗ susp_big_sep m ∗ susp_bad_ge1 m.
 
   (* Definition in_susp_table (l : loc) (id : nat) : iProp Σ :=
     ∃ (d v : val) (m : gmap val val) (s : nat),
@@ -384,32 +486,27 @@ Section proof.
       .*)
 
   Lemma v_finish_spec1 :
-    ∀ (a aᵥ aᵢ x ser : val) (st : loc) (A : lrel_bi Σ),
-      {{{ inv_susp_table st }}}
+    ∀ (a x ser : val) (st : loc),
+      {{{ True }}}
         v_finish #st a x ser
         {{{ (finish : val), RET finish;
-            finish_spec1 finish x a aᵥ aᵢ ser A }}}.
+            finish_spec1 finish x a ser }}}.
   Proof.
-    iIntros (????????) "#Htab HΦ".
+    iIntros (?????) "_ HΦ".
     rewrite /v_finish.
     wp_pures. iModIntro. iApply "HΦ".
     rewrite /finish_spec1.
-    iIntros (??????).
-    iIntros (?) "!# (Htok & % & #hashs & #Hserspec & Hserproph & Hser & #HA) HΦ".
-    (* iIntros (?) "!# (Htok & Hserproph & #HA & #Hserspec & #hashs & #Hrel_bin & #Hrel_un & #Hser & %) HΦ". *)
-    wp_pures. wp_apply ("Hserspec" with "[//] [$Hserproph $Htok]").
+    iIntros (?????).
+    iIntros (?) "!# (Htok & #Hser & #Hserspec & %) HΦ".
+    wp_pures. wp_apply ("Hserspec" with "[//] [$Hser $Htok]").
     iIntros ([]); last first.
     { iIntros "(Htok & #Hsers)". wp_pures.
-      iModIntro. iApply ("HΦ" $! None). eauto. }
-    iIntros "(Htok & #[[% #Hsers]|%])"; simplify_eq; wp_pures;
+      iModIntro. iApply ("HΦ" $! None). iFrame. }
+    iIntros "(Htok & #[[% Hsers]|%])"; simplify_eq; wp_pures;
     wp_apply (wp_hash); try done;
-    iIntros "#hashs0"; wp_pures;
-    case_bool_decide; simplify_eq; wp_pures;
-
-    destruct (decide (collision s s')) as [|Hnc%not_collision];
-      try (iExFalso; by iApply (hashes_auth.hashed_inj_or_coll with "hashs hashs0") );
-    destruct Hnc as [<-|?]; simplify_eq.
-    - iApply ("HΦ" $! (Some _)). by iFrame "∗ #".
+    iIntros "#hashs'"; wp_pures;
+    case_bool_decide; simplify_eq; wp_pures.
+    - iApply ("HΦ" $! (Some _)); by iFrame "∗ #".
     - iApply ("HΦ" $! None); by iFrame "∗ #".
 
     (* iPoseProof "HA" as "[HA_bin HA_un]".
@@ -421,160 +518,226 @@ Section proof.
     iApply ("HΦ" $! (Some _)). by iFrame "∗ #". *)
   Qed.
 
-  Lemma v_finish_spec2 :
-    ∀ (a aᵥ aᵢ x ser : val) (st : loc) (A : lrel_bi Σ),
-      {{{ inv_susp_table st }}}
+  Lemma v_finish_spec1_bad :
+    ∀ (a x ser : val) (st : loc),
+      {{{ True }}}
         v_finish #st a x ser
         {{{ (finish : val), RET finish;
-            finish_spec2 finish x a aᵥ aᵢ ser A }}}.
+            finish_spec1_bad finish x a ser }}}.
   Proof.
-    iIntros (????????) "#Htab HΦ".
+    iIntros (?????) "_ HΦ".
     rewrite /v_finish.
     wp_pures. iModIntro. iApply "HΦ".
     rewrite /finish_spec1.
-    iIntros (???????[??]).
-    iIntros (?) "!# (Htok & % & #Hserspec & #hashs & #Hinv & #Hserproph & #Hser & #HA & %) HΦ".
-    wp_pures. wp_apply ("Hserspec" with "[//] [$Hserproph $Htok]").
+    iIntros (?????).
+    iIntros (?) "!# (Htok & #Hser & #Hserspec & #hashs & % & %) HΦ".
+    wp_pures. wp_apply ("Hserspec" with "[//] [$Hser $Htok]").
     iIntros ([]); last first.
     { iIntros "(Htok & #Hsers)". wp_pures.
-      iModIntro. iApply ("HΦ" $! None). eauto. }
-    iIntros "(Htok & #[[% Hsers]|%])"; simplify_eq; wp_pures.
-    iMod (na_inv_acc with "Hinv Htok") as "(Hinv1 & Htok & Hclose)"; [solve_ndisj|solve_ndisj|].
-    iDestruct "Hinv1" as ">[(%&%& #hashs1 & %& #Hsusp & %Hser)|(%&%&%& Hsusp & Hproph & %Hser)]";
-      wp_load; wp_pures; destruct! Hser; simplify_eq.
-    - iMod ("Hclose" with "[$Htok]") as "Htok".
-      { iNext. iLeft. iFrame "hashs #". iSplit; try done.
-        iRight. repeat iExists _. iSplit; eauto. }
-      wp_apply wp_hash; try done;
-      iIntros "#hashs0"; wp_pures.
-      destruct (decide (collision s1 s)) as [|Hnc%not_collision];
-        try (iExFalso; by iApply (hashes_auth.hashed_inj_or_coll with "hashs1 hashs") );
-      destruct Hnc as [<-|?]; simplify_eq.
+      iModIntro. iApply ("HΦ" $! None). by iFrame. }
+    iIntros "(Htok & #[[% Hsers]|%])"; simplify_eq; wp_pures;
+    wp_apply (wp_hash); try done;
+    iIntros "#hashs'"; wp_pures;
+    case_bool_decide; simplify_eq; wp_pures;
 
-      case_bool_decide; simplify_eq; wp_pures;
+    destruct (decide (collision s s')) as [|Hnc%not_collision];
+      try (iExFalso; by iApply (hashes_auth.hashed_inj_or_coll with "hashs hashs'") );
+    destruct Hnc as [<-|?]; simplify_eq.
+    iApply ("HΦ" $! None); by iFrame "∗ #".
 
-      destruct (decide (collision s1 s')) as [|Hnc%not_collision];
-        try (iExFalso; by iApply (hashes_auth.hashed_inj_or_coll with "hashs1 hashs0") );
-      destruct Hnc as [<-|?]; simplify_eq.
-      + iApply ("HΦ" $! (Some _)). by iFrame "∗ #".
-      + iApply ("HΦ" $! None); by iFrame "∗ #".
-    
-    - wp_apply wp_hash; try done; iIntros "#hashs0"; wp_pures.
-      wp_apply (typed_proph_wp_resolve1 StringTypedProph with "Hproph"); try done.
-      wp_pures. iModIntro. iIntros (->). wp_pures.
+    (* iPoseProof "HA" as "[HA_bin HA_un]".
+    iMod ("Hrel_bin" with "[//] Htok [Hsers] Hser HA_bin") as "[Htok HA'_bin]".
+    { by iLeft. }
+    iMod ("Hrel_un" with "[//] Htok [Hsers] Hser HA_un") as "[Htok HA'_un]".
+    { by iLeft. }
 
-      iMod (na_inv_acc with "Htab Htok") as "(Htabo & Htok & Hclose_tab)"; [solve_ndisj|solve_ndisj|].
-      iDestruct "Htabo" as (??) "(Hl & >%Hm & #Hbigsep)".
-      wp_apply wp_hash; try done; iIntros "_"; wp_pures; wp_store.
-      iMod (pointsto_persist with "Hsusp") as "#Hsusp".
+    iApply ("HΦ" $! (Some _)). by iFrame "∗ #". *)
+  Qed.
 
-      wp_load. wp_bind (map_lookup _ _).
-      wp_apply (gwp_map_lookup with "[//]"); try done.
-      iIntros (??). destruct (m !! #pid) eqn:Hlookup;
-        simpl in H1; simplify_eq; wp_pures; last first.
-      { iMod ("Hclose_tab" with "[$Hl $Hbigsep $Htok //]") as "Htok".
-        iMod ("Hclose" with "[$Htok]") as "Htok".
-        { iNext. iLeft. iFrame "#". iSplit; eauto.
-          iRight. repeat iExists _. iSplit; eauto. }
-        iApply ("HΦ" $! None). by iFrame. }
-
-      iDestruct (big_sepM_lookup with "Hbigsep") as "[% Hs]"; [done|subst].
-      iDestruct "Hs" as (????????? Hv) 
-        "(#HA' & Hserspec' & [(%&hashs'&Hfinish)|(%&%&Hfinish&Hinvx)])";
-        destruct! Hv; simplify_eq; wp_pures;
-        case_bool_decide; simplify_eq; wp_pures; wp_load;
-        wp_bind (map_remove _ _); wp_apply (gwp_map_remove with "[//]");
-        try done; iIntros (??); wp_store; wp_pures;
-        iDestruct (big_sepM_delete _ m #pid ((#ctr, finish)%V) with "Hbigsep")
-          as "[_ #Hbigsep']"; try done.
-      1,3: (* First branch of the if *)
-        iMod ("Hclose_tab" with "[$Hl $Hbigsep' $Htok]") as "Htok".
-        1,3: iNext; iFrame "%".
-      1,2: (* refocus on first branch *)
-        iMod ("Hclose" with "[$Htok]") as "Htok";
-        try (iNext; iLeft; iFrame "hashs0 #"; iSplit; eauto;
-              iRight; repeat iExists _; iSplit; eauto);
-        wp_apply ("Hfinish" with "[] [$Htok]"); try done
-        iFrame "#"; eauto.
-      all: (* else branch *)
-        wp_load; wp_pures; wp_bind (map.map_insert _ _ _);
-        wp_apply (gwp_map_insert with "[//]"); try done;
-        iIntros (??); wp_store;
-        iDestruct (big_sepM_insert _ (delete #pid m) #pid ((#(ctr-1), finish)%V) with "[$Hbigsep']")
-          as "Hbigsep''"; try apply lookup_delete; 
-          iFrame "#"; repeat iExists _.
-        1,3: 
-          iSplit; try (iPureIntro; instantiate (1 := ctr-1); split; repeat f_equal; try lia);
-            eauto; admit. (* ctr - 1 > 0 *)
-      all:
-        iMod ("Hclose_tab" with "[$Hl $Hbigsep'' $Htok $Hfrag]") as "Htok";
-          iFrame "%";
-        iMod ("Hclose" with "[$Htok]") as "Htok";
-        try (iNext; iLeft; iFrame "hashs0 #"; iSplit; eauto;
-              iRight; repeat iExists _; iSplit; eauto);
-        iModIntro; by iApply ("HΦ" $! (Some _)).
-  Admitted.
-
-  (* Lemma v_finish_spec1_bad :
+  Lemma v_finish_spec2 :
     ∀ (a x ser : val) (st : loc),
       {{{ inv_susp_table st }}}
         v_finish #st a x ser
         {{{ (finish : val), RET finish;
-            finish_spec1_bad finish x a ser }}}.
+            finish_spec2 finish x a ser }}}.
   Proof.
     iIntros (?????) "#Htab HΦ".
     rewrite /v_finish.
     wp_pures. iModIntro. iApply "HΦ".
     rewrite /finish_spec1.
-    iIntros (?????).
-    iIntros (?) "!# (Htok & Hserproph & #Hserspec & #hashs & % & Hval) HΦ".
-    wp_pures. wp_apply ("Hserspec" with "[//] [$Hserproph $Htok]").
+    iIntros (s' s'' ????[??]).
+    iIntros (?) "!# (Htok & #Hser & #Hserspec & [Hpos %Ho'] & % & #Hinv) HΦ".
+    wp_pures. wp_apply ("Hserspec" with "[//] [$Hser $Htok]").
     iIntros ([]); last first.
     { iIntros "(Htok & #Hsers)". wp_pures.
-      iModIntro. iApply ("HΦ" $! None). eauto. }
-    iDestruct "Hval" as "[%|(%&%& Hsusp)]";
-      iIntros "(Htok & #[[% Hsers]|%])"; simplify_eq; wp_pures; [|wp_load; wp_pures];
-      wp_apply (wp_hash); try done; iIntros "#hashs0"; wp_pures;
-
-      destruct (decide (collision s1 s2)) as [|Hnc%not_collision];
-        try ( iExFalso; by iApply (hashes_auth.hashed_inj_or_coll with "hashs0 hashs"));
-        destruct Hnc as [<-|?]; simplify_eq;
-        case_bool_decide; wp_pures; simplify_eq;
-        iApply ("HΦ" $! None); eauto.
-  Qed. *)
+      iModIntro. iApply ("HΦ" $! None). iFrame. }
+    iIntros "(Htok & #[[% Hsers]|%])"; simplify_eq; wp_pures.
     
-  (* Lemma v_finish_spec2 :
-    ∀ (a x aᵥ aᵢ ser : val) (st : loc) (A : lrel Σ),
-      {{{ inv_susp_table st }}}
-        v_finish #st a x ser 
-      {{{ (finish : val), RET finish;
-          finish_spec2 finish x a aᵥ aᵢ ser A }}}.
+    iMod (na_inv_acc with "Htab Htok") as "(Htabo & Htok & Hclose_tab)"; [solve_ndisj|solve_ndisj|].
+    iMod (na_inv_acc with "Hinv Htok") as "(Hinv1 & Htok & Hclose)"; [solve_ndisj|solve_ndisj|].
+    
+    iDestruct "Hinv1" as ">[(%s1&%& #hashs1 & %& #Hsusp & %Hser)|(%&%&%& Hsusp & Hproph & %Hser)]";
+      wp_load; wp_pures; destruct! Hser; simplify_eq.
+    - iMod ("Hclose" with "[$Htok]") as "Htok".
+      { iNext. iLeft. iFrame "#". iSplit; eauto. 
+        iRight. repeat iExists _. iSplit; eauto. }
+      iMod ("Hclose_tab" with "[$Htok $Htabo]") as "Htok".
+      wp_apply wp_hash; try done;
+      iIntros "#hashs'"; wp_pures;
+      case_bool_decide; simplify_eq; wp_pures.
+      + iApply ("HΦ" $! (Some _)); by iFrame "∗ #".
+      + iApply ("HΦ" $! None); by iFrame "∗ #".
+    
+    - wp_apply wp_hash; try done; iIntros "#hashs'"; wp_pures.
+      wp_apply (typed_proph_wp_resolve1 StringTypedProph with "Hproph"); try done.
+      wp_pures. iModIntro. iIntros (?). wp_pures.
+
+      iDestruct "Htabo" as (??) "(Hl & %Hm & Hbigsep & Hge)".
+      wp_apply wp_hash; try done; iIntros "_"; wp_pures; wp_store.
+      iMod (pointsto_persist with "Hsusp") as "#Hsusp".
+
+      wp_load. wp_bind (map_lookup _ _).
+      wp_apply (gwp_map_lookup with "[//]"); try done.
+      iIntros (? Hl). destruct (m !! #pid) eqn:Hlookup;
+        simpl in Hl; simplify_eq; wp_pures; last first.
+      { iMod ("Hclose" with "[$Htok]") as "Htok".
+        { iNext. iLeft. iFrame "#". iSplit; eauto.
+          iRight. repeat iExists _. iSplit; eauto. }
+        iMod ("Hclose_tab" with "[$Hl $Hbigsep $Htok $Hge //]") as "Htok".
+        iApply ("HΦ" $! None). by iFrame. }
+
+      iDestruct (big_sepM_lookup_acc with "Hbigsep") as "[[% Hs] Hbigsep]"; [done|subst].
+      iDestruct "Hs" as (?????? Hv) 
+        "(#Hser' & #Hserspec' & [#Hfinish|(%&Hfrag&#Hfinish)])"; last first;
+        destruct! Hv; simplify_eq; wp_pures.
+      + destruct Ho' as [-> | ->];
+        iPoseProof (pos_auth_frag_valid with "Hpos Hfrag") as (?) "[Hpos #Hfrag]";
+        simplify_eq; first admit; clear H2.
+        iDestruct "Hge" as "[Hpos'|[Hpos'|[Hpos' %Hge]]]";
+          iPoseProof (pos_agree with "Hpos Hpos'") as (?) "[Hpos Hpos']"; 
+          simplify_eq.
+
+        case_bool_decide; simplify_eq; wp_pures; wp_load;
+          wp_bind (map_remove _ _); wp_apply (gwp_map_remove with "[//]");
+          try done; iIntros (??); wp_store; wp_pures;
+          iPoseProof ("Hbigsep" with "[$Hser' $Hserspec' $Hfinish]") as "Hbigsep";
+            try (iFrame; iExists ctr; iSplit; try done; iRight; iFrame "#");
+          iDestruct (big_sepM_delete _ m #pid ((#ctr, finish)%V) with "Hbigsep")
+            as "[_ Hbigsep']"; try done.
+        * iMod (pos_update2 with "Hpos Hpos'") as "(Hpos & Hpos' & _)".
+          iMod ("Hclose" with "[$Htok]") as "Htok";
+          try (iNext; iLeft; iFrame "hashs' #"; iSplit; eauto;
+                iRight; repeat iExists _; iSplit; eauto);
+          iMod ("Hclose_tab" with "[$Hl $Hbigsep' $Htok Hpos']") as "Htok";
+          try (iNext; iSplit; try done; iRight; by iLeft).
+          iDestruct "Hfinish" as 
+            "[(%&#hashs&[Hfinish %])|(%&%&%&#hashs&%&#Hinv'&[Hfinish %])]";
+          wp_apply ("Hfinish" with "[] [$Htok]");
+          try solve_ndisj; iFrame "# ∗"; eauto;
+          iIntros (?) "[Htok ->]"; iApply ("HΦ" $! None); by iFrame.
+        * wp_load; wp_pures; wp_bind (map.map_insert _ _ _);
+          wp_apply (gwp_map_insert with "[//]"); try done;
+          iIntros (??); wp_store;
+          iDestruct (big_sepM_insert _ (delete #pid m) #pid ((#(ctr-1), finish)%V) with "[$Hbigsep']")
+            as "Hbigsep''"; try apply lookup_delete; iFrame "#".
+          { iExists (ctr-1). iPureIntro. split; repeat f_equal; try lia. admit. }
+          iMod ("Hclose" with "[$Htok]") as "Htok";
+            try (iNext; iLeft; iFrame "hashs' #"; iSplit; eauto;
+                  iRight; repeat iExists _; iSplit; eauto).
+          iMod ("Hclose_tab" with "[$Hl $Hbigsep'' $Htok Hpos']") as "Htok"; iFrame "%".
+          { iNext. do 2 iRight. iFrame. admit. }
+          iModIntro; iApply ("HΦ" $! (Some _)); by iFrame.
+      + case_bool_decide; simplify_eq; wp_pures; wp_load;
+          wp_bind (map_remove _ _); wp_apply (gwp_map_remove with "[//]");
+          try done; iIntros (??); wp_store; wp_pures;
+          iPoseProof ("Hbigsep" with "[$Hser' $Hserspec']") as "Hbigsep";
+            repeat (iExists _); try (iSplit). 1,4: admit.
+          1,3: by iLeft.
+        all:
+          iDestruct "Hfinish" as 
+            "[(%&%&Hfinish)|(%&%&%&#Hinv'&Hfinish)]";
+          iDestruct (big_sepM_delete _ m #pid ((#ctr, finish)%V) with "Hbigsep")
+            as "[_ Hbigsep]"; try done.
+        1,2: (* First branch of the if *)
+          iMod ("Hclose" with "[$Htok]") as "Htok";
+          try (iNext; iLeft; iFrame "hashs' #"; iSplit; eauto;
+                iRight; repeat iExists _; iSplit; eauto);
+          destruct Ho' as [-> | ->];
+            iDestruct "Hge" as "[Hpos'|[Hpos'|[Hpos' %Hge]]]";
+            iPoseProof (pos_agree with "Hpos Hpos'") as (?) "[Hpos Hpos']"; 
+            simplify_eq;
+          iMod ("Hclose_tab" with "[$Hl $Hbigsep $Htok Hpos']") as "Htok";
+            try (iFrame "%"; iNext; iFrame; eauto; admit).
+          1,2: 
+            wp_apply ("Hfinish" with "[//] [$Htok $Hser' $Hserspec' //]");
+            iIntros (?) "Htok"; iApply "HΦ"; iFrame; destruct o; eauto;
+              try (by iLeft); by iRight.
+          1,2: 
+            wp_apply ("Hfinish" with "[//] [$Htok $Hser' $Hserspec' $Hinv' $Hpos]");
+              eauto.
+        all: (* else branch *)
+          wp_load; wp_pures; wp_bind (map.map_insert _ _ _);
+          wp_apply (gwp_map_insert with "[//]"); try done;
+          iIntros (??); wp_store;
+          iDestruct (big_sepM_insert _ (delete #pid m) #pid ((#(ctr-1), finish)%V) with "[$Hbigsep]")
+            as "Hbigsep"; try apply lookup_delete;
+          try (iFrame "Hser' Hserspec'"); repeat iExists _; try (iSplit). 1,4: admit.
+        1,3 : iLeft; iFrame "#"; eauto.
+        all:
+          iMod ("Hclose" with "[$Htok]") as "Htok";
+          try (iNext; iLeft; iFrame "hashs' #"; iSplit; eauto;
+                iRight; repeat iExists _; iSplit; eauto);
+          destruct Ho' as [-> | ->];
+            iDestruct "Hge" as "[Hpos'|[Hpos'|[Hpos' %Hge]]]";
+            iPoseProof (pos_agree with "Hpos Hpos'") as (?) "[Hpos Hpos']"; 
+            simplify_eq;
+          iMod ("Hclose_tab" with "[$Hl $Hbigsep $Htok Hpos']") as "Htok";
+            try (iFrame "%"; iNext; iFrame; eauto; admit);
+          iModIntro; iApply ("HΦ" $! (Some _)); by iFrame.
+  Admitted.
+
+  Lemma v_finish_spec2_bad :
+    ∀ (a x ser : val) (st : loc),
+      {{{ True }}}
+        v_finish #st a x ser
+        {{{ (finish : val), RET finish;
+            finish_spec2_bad finish x a ser }}}.
   Proof.
-    iIntros (????????) "#Htab HΦ".
+    iIntros (????? _ ) "HΦ".
     rewrite /v_finish.
     wp_pures. iModIntro. iApply "HΦ".
-    rewrite /finish_spec2.
-    iIntros (?????).
-    iIntros (??) "!# (Htok & Hcount & #HA & #Hserspec & #Hrel & #hashs2 & #Hser & % & #Hsusp) HΦ".
-    wp_pures. wp_apply ("Hserspec" with "[$Hcount $Htok]").
+    rewrite /finish_spec1.
+    iIntros (s s' s'' ????).
+    iIntros (?) "!# (Htok & #Hser & #Hserspec & % & % & #hashs & #Hinv & %) HΦ".
+    wp_pures. wp_apply ("Hserspec" with "[//] [$Hser $Htok]").
     iIntros ([]); last first.
     { iIntros "(Htok & #Hsers)". wp_pures.
-      iModIntro. iApply ("HΦ" $! None). eauto. }
-    iIntros "(Htok & #Hsers)". wp_pures.
-    simplify_eq. wp_pures. wp_load. wp_pures.
-    wp_apply (wp_hash); try done.
-    iIntros "#hashs". wp_pures.
-    case_bool_decide; simplify_eq; wp_pures;
-      try ( iApply ("HΦ" $! None); eauto ).
+      iModIntro. iApply ("HΦ" $! None). by iFrame. }
+    iIntros "(Htok & #[[% Hsers]|%])"; simplify_eq; wp_pures.
+    iMod (na_inv_acc with "Hinv Htok") as "(Hinv1 & Htok & Hclose)"; [solve_ndisj|solve_ndisj|].
+    iDestruct "Hinv1" as ">[(%s1&%& #hashs1 & %& #Hsusp & %Hser)|(%&%&%& Hsusp & Hproph & %Hser)]";
+      wp_load; wp_pures; destruct! Hser; simplify_eq.
+    - assert (s = s1) as ->; first admit.
+      iMod ("Hclose" with "[$Htok]") as "Htok".
+      { iNext. iLeft. iFrame "#". iSplit; eauto. 
+        iRight. repeat iExists _. iSplit; eauto. }
+      wp_apply wp_hash; try done;
+      iIntros "#hashs'"; wp_pures;
+      case_bool_decide; simplify_eq; wp_pures;
 
-    destruct (decide (collision s s2)) as [|Hnc%not_collision];
-      try (iExFalso; by iApply (hashes_auth.hashed_inj_or_coll with "hashs hashs2") ).
-    destruct Hnc as [<-|?]; simplify_eq.
-    iApply ("HΦ" $! (Some _)).
-    iFrame.
-    iModIntro. iIntros (->).
-    iApply (evi_type_ser''_inj authBaseN); [by iLeft|done].
-  Qed. *)
+      destruct (decide (collision s' s1)) as [|Hnc%not_collision];
+        try (iExFalso; by iApply (hashes_auth.hashed_inj_or_coll with "hashs' hashs1") );
+      destruct Hnc as [<-|?]; simplify_eq.
+      iApply ("HΦ" $! None); by iFrame "∗ #".
+    
+    - wp_apply wp_hash; try done; iIntros "#hashs'"; wp_pures.
+      wp_apply (typed_proph_wp_resolve1 StringTypedProph with "Hproph"); try done.
+      wp_pures. iModIntro. iIntros (?). wp_pures.
+
+      destruct (decide (collision s s')) as [|Hnc%not_collision];
+        try (iExFalso; by iApply (hashes_auth.hashed_inj_or_coll with "hashs hashs'") );
+      destruct Hnc as [<-|?]; simplify_eq.
+  Admitted.
 
   Definition is_proof (v : val) : iProp Σ :=
     ∃ (l : list string), ⌜is_list l v⌝.
@@ -592,26 +755,29 @@ Section proof.
 
   Definition lrel_bin_auth_comp' (A : lrel_bi Σ) : lrel Σ := LRel (λ v1 v2,
     ∀ t K (w w' : val) (cntr : nat),
-      {{{ spec_ideal t (fill K (v2 w')) ∗ seq_tok ⊤ ∗ is_proof_state w cntr ∗ idcntr_frag cntr }}}
+      {{{ spec_ideal t (fill K (v2 w')) ∗ seq_tok ⊤ ∗ 
+          is_proof_state w cntr ∗ good_pos }}}
         v1 w
       {{{ (o1 : option val), RET $o1;
           seq_tok ⊤ ∗
             if o1 is Some w1 then
               ∃ (a prfst prf : val) (cntr' : nat),
-                 ⌜w1 = (prfst, a)%V ∧ prfst = (prf, #cntr')%V⌝ ∗ idcntr_frag cntr' ∗
-                  ((∃ (w2 : val), spec_ideal t (fill K w2) ∗ lrel_auth_comp_post A w1 w2) ∨ lrel_auth_comp_post_bad (lrel_bi_un A) w1)
+                 ⌜w1 = (prfst, a)%V ∧ prfst = (prf, #cntr')%V⌝ ∗
+                  ((∃ (w2 : val), spec_ideal t (fill K w2) ∗ 
+                    lrel_auth_comp_post A w1 w2 ∗ good_pos) ∨ 
+                    lrel_auth_comp_post_bad (lrel_bi_un A) w1 ∗ bad_pos)
             else True }}})%I.
 
   Definition lrel_un_auth_comp' (A_un : lrel_un Σ) : lrel_un Σ := LRelUn (λ v1,
     ∀ (w : val) (cntr : nat),
-      {{{ seq_tok ⊤ ∗ is_proof_state w cntr ∗ idcntr_frag cntr }}}
+      {{{ seq_tok ⊤ ∗ is_proof_state w cntr ∗ bad_pos }}}
         v1 w
       {{{ (o1 : option val), RET $o1;
           seq_tok ⊤ ∗
             if o1 is Some w1 then
               ∃ (a prfst prf : val) (cntr' : nat),
-                ⌜w1 = (prfst, a)%V ∧ prfst = (prf, #cntr')%V⌝ ∗ idcntr_frag cntr' ∗
-                  lrel_auth_comp_post_bad A_un w1
+                ⌜w1 = (prfst, a)%V ∧ prfst = (prf, #cntr')%V⌝ ∗
+                  lrel_auth_comp_post_bad A_un w1 ∗ bad_pos
             else True }}})%I.
 
   (* Definition lrel_auth_comp_bad : lrel Σ := LRel (λ v1 v2,
@@ -651,7 +817,7 @@ Section proof.
   Proof.
     iIntros "#HA".
     rewrite interp_var1_ext2.
-    iIntros (?? Ψ) "!# (Htok & %H & Hid) HΨ".
+    iIntros (?? Ψ) "!# (Htok & %H & ?) HΨ".
     simpl in H. destruct H as (? & -> & Hp).
     wp_pures. iModIntro. iApply ("HΨ" $! (Some _)).
     iFrame "Htok". iExists _, _, _, _.
@@ -677,7 +843,7 @@ Section proof.
         iModIntro. iFrame. clear.
         iSplit; interp_unfold!.
         { rewrite interp_var1_ext2.
-          iIntros (????? Ψ) "!# (Hi & Htok & %H & Hid) HΨ".
+          iIntros (????? Ψ) "!# (Hi & Htok & %H & ?) HΨ".
           simpl in H. destruct H as (? & -> & Hp).
           i_pures; wp_pures.
           iModIntro. iApply ("HΨ" $! (Some _)).
@@ -716,14 +882,14 @@ Section proof.
   Proof.
     iIntros "#HmA #HmB".
     rewrite interp_var2_ext3. 
-    iIntros (???Ψ) "!# [Htok [#Hprf Hid]] HΨ". wp_pures.
+    iIntros (???Ψ) "!# (Htok & #Hprf & Hpos) HΨ". wp_pures.
     wp_pures. wp_bind (v _)%I.
-    wp_apply ("HmA" with "[$Htok $Hprf $Hid]").
+    wp_apply ("HmA" with "[$Htok $Hprf $Hpos]").
     iIntros (o) "[Htok Ho]".
     destruct o; last first.
     { wp_pures. iApply ("HΨ" $! None). by iFrame. }
     iPoseProof "Hprf" as (??) "Hprf'". 
-    iDestruct "Ho" as (????[??]) "[Hid (%&%&%&%& #Hprf1 & HA)]".
+    iDestruct "Ho" as (????[??]) "[(%&%&%&%& #Hprf1 & HA) Hpos]".
     iPoseProof "Hprf1" as (??) "Hprf1'". 
     simplify_eq. wp_pures.
     rewrite interp_un_arr_unfold.
@@ -733,7 +899,7 @@ Section proof.
     iIntros (?) "(H & Htok) /=".
     interp_unfold in "H".
     rewrite interp_var2_ext3.
-    wp_apply ("H" with "[$Htok $Hprf1 $Hid]").
+    wp_apply ("H" with "[$Htok $Hprf1 $Hpos]").
     iIntros (?) "(Htok & Ho) /=".
     iApply "HΨ". iFrame.
   Qed.
@@ -766,16 +932,16 @@ Section proof.
             interp_unfold in "HmA".
             iSplit; interp_unfold!.
             { rewrite interp_var2_ext3.
-              iIntros (u1 u2 ??? Ψ) "!# (Hi & Htok & Hprf & Hid) HΨ".
+              iIntros (u1 u2 ??? Ψ) "!# (Hi & Htok & Hprf & Hpos) HΨ".
               i_pures; wp_pures.
               i_bind (v2 _)%I; wp_bind (v1 _)%I.
               iDestruct "HmA" as "[HmA _]".
-              wp_apply ("HmA" with "[$Hi $Htok $Hprf $Hid]").
+              wp_apply ("HmA" with "[$Hi $Htok $Hprf $Hpos]").
               iIntros (o) "[Htok Ho]".
               destruct o; last first.
               { wp_pures. iApply ("HΨ" $! None). by iFrame. }
-              iDestruct "Ho" as (????) "(%H & Hid & [H|H])".
-              + iDestruct "H" as (?) "[Hi H]".
+              iDestruct "Ho" as (????) "(%H & [H|H])".
+              + iDestruct "H" as (?) "(Hi & H & Hpos)".
                 iDestruct "H" as (? a1' a2 ->) "[#Hprf #HA]".
                 wp_pures.
                 wp_bind (w1 _)%E; i_bind (w2 _ )%E.
@@ -788,10 +954,11 @@ Section proof.
                 iPoseProof "Hprf" as (??) "Hprf'". simplify_eq.
                 interp_unfold in "H". rewrite interp_var2_ext3.
                 iDestruct "H" as "[H _]".
-                wp_apply ("H" with "[$Hi $Htok $Hprf $Hid]").
+                wp_apply ("H" with "[$Hi $Htok $Hprf $Hpos]").
                 iIntros (?) "(Htok & Ho) /=".
                 iApply "HΨ". iFrame.
-              + iDestruct "H" as (??? ->) "(#Hprf & #HA)".
+              + iDestruct "H" as "[H Hpos]".
+                iDestruct "H" as (??? ->) "(#Hprf & #HA)".
                 wp_pures.
                 wp_bind (w1 _)%E.
                 iDestruct "HmB" as "[_ HmB]".
@@ -804,11 +971,11 @@ Section proof.
                 destruct! H. simplify_eq.
                 iPoseProof "Hprf" as (??) "Hprf'". simplify_eq.
                 rewrite interp_var2_ext3.
-                wp_apply ("H" with "[$Htok $Hprf $Hid]").
+                wp_apply ("H" with "[$Htok $Hprf $Hpos]").
                 iIntros (?) "(Htok & Ho) /=".
                 iApply "HΨ". iFrame.
                 destruct o1; last done. iFrame.
-                iDestruct "Ho" as (????[??]) "[Hbad Hid]".
+                iDestruct "Ho" as (????[??]) "Hbad".
                 iExists _, _, _, _. iSplit; first done.
                 iFrame. }
             { iDestruct "HmA" as "[_ HmA]".
@@ -860,6 +1027,208 @@ Section proof.
       iApply (refines_un_auth_bind with "HmA HmB"). }
   Qed.
 
+  Lemma refines_un_auth_unauth c :
+    ∀ (ser deser count v : val) tA' A,
+    inv_susp_table c -∗
+    ser_spec_un (lrel_bi_un A) ser tA' -∗
+    ser_spec_3 ser tA' -∗
+    count_spec count tA' -∗
+    deser_spec authBaseN (lrel_bi_un A) deser tA' -∗
+    auth_some_un authBaseN (lrel_bi_un A) v -∗
+    lrel_bi_un (lrel_auth_comp A)
+      (λ: "proof",
+        match: InjRV v with
+          InjL <> => InjL #()
+        | InjR "a" =>
+          let: "counter" := "proof" in
+          let: "pf_stream" := Fst "counter" in
+          let: "counter" := Snd "counter" in
+          match: list_head "pf_stream" with
+            InjL <> => InjL #()
+          | InjR "p" =>
+            let: "id" := "counter" in
+            let: "serialize" := (ser, deser, count)%V in
+            let: "deserialize" := Snd (Fst "serialize") in
+            let: "count" := Snd "serialize" in
+            let: "serialize" := Fst (Fst "serialize") in
+            match: "deserialize" "id" "p" with
+              InjL <> => InjL #()
+            | InjR "x" =>
+              let: "nchild" := "count" "x" in
+              let: "finish" := v_finish #c "a" "x" "serialize" in
+              match: if: "nchild" = #0 then "finish" #() else #c <- map.map_insert "id" ("nchild", "finish") ! #c;;  InjRV #() with
+                InjL <> => InjL #()
+              | InjR <> => InjR (list_tail "pf_stream", "id" + #1, "x")
+              end
+            end
+          end
+        end)%V.
+  Proof.
+    iIntros (??????) "#Htab #Hser' #Hser3 #Hcount #Hdeser #Hauth_un".
+    iIntros (???) "!# (Htok & Hproof & Hpos) HΦ".
+    wp_pures.
+    iDestruct "Hproof" as (? -> ) "Hproof".
+    wp_pures. iDestruct "Hproof" as "(% & %)".
+    wp_apply gwp_list_head; [done| ].
+    iIntros (vl [[-> ->] | (s1' &?& -> & -> )]).
+    { wp_pures. iModIntro.
+      iApply ("HΦ" $! None). iFrame. }
+
+    wp_pures. wp_apply "Hdeser"; [done|].
+    iIntros (?) "Hdepar".
+    wp_apply "Hdepar"; [done|].
+    iIntros ([]); last first.
+    { iIntros "_". wp_pures. iApply ("HΦ" $! None). iFrame. eauto. }
+    
+    iPoseProof "Hauth_un" as "[(%&%)|(%&%&%&#Hinv)]";
+      simplify_eq; iIntros "[Hserser Hserproph]";
+      iPoseProof ("Hserproph" with "Hserser") as ">[#HA_un [%s2 #Hserproph]]";
+      wp_pures; wp_apply ("Hcount" $! _ _ ⊤ with "[//] [$Hserproph $Htok]");
+      iIntros (?) "[_ Htok]"; wp_pures.
+    - wp_apply v_finish_spec1; try done.
+      iIntros (finish) "Hfinish". wp_pures.
+
+      case_bool_decide; wp_pures; simplify_eq.
+      + wp_bind (finish #()).
+        assert (c0 = 0); [lia|]. simplify_eq.
+
+        iApply ("Hfinish" $! _ _ ⊤ with "[//] [$Htok $Hserproph $Hser3 //]").
+        iNext. iIntros ([]) "Htok"; wp_pures; last first.
+        { iApply ("HΦ" $! (None)). by iFrame. }
+
+        wp_apply gwp_list_tail; [done|].
+        iIntros (vl Hl).
+
+        (* iMod (na_inv_acc with "Htab Htok") as "(Htabo & Htok & Hclose_tab)"; [solve_ndisj|solve_ndisj|]. *)
+        (* iDestruct "Htabo" as (??) "(Hl & >%Hm & Hbigsep)". *)
+        wp_pures.
+
+        (* iPoseProof (idcntr_agree with "[$Hid $Hfrag]") as (->) "[Hid Hfrag]".
+        iMod (idcntr_update with "[$Hid $Hfrag]") as "[Hid Hfrag]". *)
+
+        (* iPoseProof (idcntr_agree with "[$Hst $Hfrag]") as (->) "[Hst Hfrag]".
+        iMod (global_state_update_empty with "[$Hst $Hfrag]") as "[Hst Hfrag]". *)
+        
+        (* iMod ("Hclose_tab" with "[$Hl $Hbigsep $Htok]") as "Htok"; try done. *)
+        (* { iFrame "%". iPureIntro. intros ?. apply Hci. lia. } *)
+        
+        iApply ("HΦ" $! (Some _)).
+
+        iFrame "# ∗"; iModIntro; repeat (iExists _);
+          iSplit; try (iSplit; try done; iPureIntro; repeat f_equal; 
+            instantiate (1 := cntr + 1); lia);
+          iFrame "# ∗ %"; iExists _, (cntr+1);
+          iSplit; iPureIntro; repeat f_equal; lia.
+
+      + iMod (na_inv_acc with "Htab Htok") as "(Htabo & Htok & Hclose_tab)"; [solve_ndisj|solve_ndisj|].
+        iDestruct "Htabo" as (??) "(Hl & >%Hm & Hbigsep & Hge)". wp_load.
+
+        (* iPoseProof (idcntr_agree with "[$Hst $Hfrag]") as (->) "[Hst Hfrag]".
+        iPoseProof (msize_agree with "[$Hms $Hs]") as (<-) "[Hms Hs]".
+        iMod (global_state_update_singleton with "[$Hst $Hfrag]") as "(Hst & Hins & Hfrag)". *)
+        (* iPoseProof (idcntr_agree with "[$Hid $Hfrag]") as (->) "[Hid Hfrag]".
+        iMod (idcntr_update with "[$Hid $Hfrag]") as "[Hid Hfrag]". *)
+
+        (* assert (m0 !! #c1 = None). { apply Hci. lia. } *)
+        wp_bind (map.map_insert _ _ _). wp_pures.
+        iApply (gwp_map_insert #cntr (#c0, finish)%V d m _ _); [done|done|].
+        
+        iModIntro. iIntros (d') "%Hmap'". wp_store.
+        (* iMod (msize_update _ (s+1) with "[$Hms $Hs]") as "[Hms Hs]". *)
+        wp_pures. wp_apply (gwp_list_tail with "[//]").
+        iIntros "/=" (tl Htl). wp_pures.
+        iDestruct "Hge" as "[Hpos'|[Hpos'|[Hpos' %Hge]]]";
+          iPoseProof (pos_agree with "Hpos Hpos'") as (?) "[Hpos Hpos']"; 
+          simplify_eq.
+
+        iMod ("Hclose_tab" with "[$Hl Hbigsep Hpos' $Htok Hfinish]") as "Htok".
+        { iNext. iExists _. iSplit; try done. iSplit; last admit.
+          iApply (big_sepM_insert_2 with "[Hfinish]"); last done.
+          assert (c0 > 0).
+          { apply Nat.neq_0_lt_0. intros ->. by apply H0. }
+          repeat iExists _. repeat (try (iSplit; eauto)).
+          do 2 iLeft. iFrame. eauto. }
+
+        iApply ("HΦ" $! (Some _)).
+        iFrame "# ∗"; iModIntro; repeat (iExists _);
+          iSplit; try (iSplit; try done; iPureIntro; repeat f_equal; 
+            instantiate (1 := cntr + 1); lia);
+          iFrame "# ∗ %"; iExists _, (cntr+1);
+          iSplit; iPureIntro; repeat f_equal; lia.
+    
+    - wp_apply (v_finish_spec2 with "Htab").
+      iIntros (finish) "Hfinish". wp_pures.
+
+      case_bool_decide; wp_pures; simplify_eq.
+      * wp_bind (finish #()).
+        assert (c0 = 0); [lia|]. simplify_eq.
+        
+        iApply ("Hfinish" $! _ _ ⊤ tA' with "[//] [$Htok $Hserproph $Hser3 $Hinv $Hpos]"); eauto.
+        iNext. iIntros ([]) "[Htok Hpos]"; wp_pures; last first.
+        { iApply ("HΦ" $! (None)). eauto. }
+
+        wp_apply gwp_list_tail; [done|].
+        iIntros (vl Hl).
+
+        (* iMod (na_inv_acc with "Htab Htok") as "(Htabo & Htok & Hclose_tab)"; [solve_ndisj|solve_ndisj|]. *)
+        (* iDestruct "Htabo" as (??) "(Hl & >%Hm & Hbigsep)". *)
+        wp_pures.
+
+        (* iPoseProof (idcntr_agree with "[$Hid $Hfrag]") as (->) "[Hid Hfrag]".
+        iMod (idcntr_update with "[$Hid $Hfrag]") as "[Hid Hfrag]". *)
+
+        (* iPoseProof (idcntr_agree with "[$Hst $Hfrag]") as (->) "[Hst Hfrag]".
+        iMod (global_state_update_empty with "[$Hst $Hfrag]") as "[Hst Hfrag]". *)
+        
+        (* iMod ("Hclose_tab" with "[$Hl $Hbigsep $Htok]") as "Htok"; try done. *)
+        (* { iFrame "%". iIntros (id). iPureIntro. intros ?. apply Hci. lia. } *)
+        
+        iApply ("HΦ" $! (Some _)).
+
+        iFrame "# ∗"; iModIntro; repeat (iExists _);
+          iSplit; try (iSplit; try done; iPureIntro; repeat f_equal; 
+            instantiate (1 := cntr + 1); lia);
+          iFrame "# ∗ %". iExists _, (cntr+1);
+          iSplit; iPureIntro; repeat f_equal; lia.
+      
+      * iMod (na_inv_acc with "Htab Htok") as "(Htabo & Htok & Hclose_tab)"; [solve_ndisj|solve_ndisj|].
+        iDestruct "Htabo" as (??) "(Hl & >%Hm & Hbigsep & Hge)". wp_load.
+
+        (* iPoseProof (idcntr_agree with "[$Hst $Hfrag]") as (->) "[Hst Hfrag]".
+        iPoseProof (msize_agree with "[$Hms $Hs]") as (<-) "[Hms Hs]".
+        iMod (global_state_update_singleton with "[$Hst $Hfrag]") as "(Hst & Hins & Hfrag)". *)
+        (* iPoseProof (idcntr_agree with "[$Hid $Hfrag]") as (->) "[Hid Hfrag]".
+        iMod (idcntr_update with "[$Hid $Hfrag]") as "[Hid Hfrag]". *)
+
+        (* assert (m0 !! #c1 = None). { apply Hci. lia. } *)
+        wp_bind (map.map_insert _ _ _). wp_pures.
+        iApply (gwp_map_insert #cntr (#c0, finish)%V d m _ _); [done|done|].
+        
+        iModIntro. iIntros (d') "%Hmap'". wp_store.
+        (* iMod (msize_update _ (s+1) with "[$Hms $Hs]") as "[Hms Hs]". *)
+        wp_pures. wp_apply (gwp_list_tail with "[//]").
+        iIntros "/=" (tl Htl). wp_pures.
+        iDestruct "Hge" as "[Hpos'|[Hpos'|[Hpos' %Hge]]]";
+          iPoseProof (pos_agree with "Hpos Hpos'") as (?) "[Hpos Hpos']"; 
+          simplify_eq.
+
+        iMod ("Hclose_tab" with "[$Hl Hbigsep Hpos' $Htok Hfinish]") as "Htok".
+        { iNext. iExists _. iSplit; try done. iSplit; last admit.
+          iApply (big_sepM_insert_2 with "[Hfinish]"); last done.
+          assert (c0 > 0).
+          { apply Nat.neq_0_lt_0. intros ->. by apply H0. }
+          repeat iExists _. repeat (try (iSplit; [done|])).
+          iLeft. iRight. by iFrame "# ∗". }
+
+        iApply ("HΦ" $! (Some _)).
+
+        iFrame "# ∗"; iModIntro; repeat (iExists _);
+          iSplit; try (iSplit; try done; iPureIntro; repeat f_equal; 
+            instantiate (1 := cntr + 1); lia);
+          iFrame "# ∗ %"; iExists _, (cntr+1);
+          iSplit; iPureIntro; repeat f_equal; lia.
+  Admitted.
+
   Lemma refines_auth_unauth Θ (Δ : ctxO Σ Θ) c :
     inv_susp_table c
     ⊢ REL v_unauth #c << i_unauth :
@@ -889,16 +1258,16 @@ Section proof.
           iDestruct "Hauth_bi" as "[(% & -> & Hauth_bi)|->]"; wp_pures; last first.
           { iFrame. iModIntro.
             interp_unfold!. rewrite interp_var2_ext3. iSplit.
-            { iIntros (??????) "!# (Hi & Htok & Hproof & Hid) HΦ".
+            { iIntros (??????) "!# (Hi & Htok & Hproof & Hpos) HΦ".
               wp_pures. iApply ("HΦ" $! None). by iFrame. }
-            iIntros (???) "!# (Htok & Hproof) HΦ".
+            iIntros (???) "!# (Htok & Hproof & Hpos) HΦ".
             wp_pures. iApply ("HΦ" $! None). by iFrame. }
           iDestruct "Hauth_un" as "[(% & % & Hauth_un)|->]"; last first.
           { iFrame. iModIntro.
             interp_unfold!. rewrite interp_var2_ext3. iSplit.
-            { iIntros (??????) "!# (Hi & Htok & Hproof & Hid) HΦ".
+            { iIntros (??????) "!# (Hi & Htok & Hproof & Hpos) HΦ".
               wp_pures. iApply ("HΦ" $! None). by iFrame. }
-            iIntros (???) "!# (Htok & Hproof) HΦ".
+            iIntros (???) "!# (Htok & Hproof & Hpos) HΦ".
             wp_pures. iApply ("HΦ" $! None). by iFrame. }
 
           iDestruct "Hevi" as "[Hrel Hevi_un]".    
@@ -906,7 +1275,7 @@ Section proof.
           simplify_eq.
           iFrame. iModIntro.
           iSplit; interp_unfold!; rewrite interp_var2_ext3.
-          { iIntros (??????) "!# (Hi & Htok & Hproof & Hid) HΦ".
+          { iIntros (??????) "!# (Hi & Htok & Hproof & Hpos) HΦ".
             wp_pures. i_pures. iDestruct "Hproof" as (? -> ) "Hproof".
             wp_pures. iDestruct "Hproof" as "(% & %)".
             wp_apply gwp_list_head; [done| ].
@@ -920,180 +1289,271 @@ Section proof.
             iIntros ([]); last first.
             { iIntros "_". wp_pures. iApply ("HΦ" $! None). iFrame. eauto. }
             
-            iPoseProof "Hauth_bi" as "(%&%&%&#Hser1&#HA&[(#hashs1&%)|(%&%&%&%&Hinv)])";
+            iPoseProof "Hauth_bi" as "(%&%&%&#hashs1&#Hser1&#HA&[%|(%&%&%&%&#Hinv)])";
               simplify_eq; iIntros "[Hserser Hserproph]";
               iPoseProof ("Hserproph" with "Hserser") as ">[#HA_un [%s2 #Hserproph]]";
               wp_pures; wp_apply ("Hcount" $! _ _ ⊤ with "[//] [$Hserproph $Htok]");
               iIntros (?) "[_ Htok]"; wp_pures.
             - (* iPoseProof (deser_ser_proph authBaseN with "[$Htok $Hserser]") as ">[Htok [% Hserproph]]". *)
-              wp_apply (v_finish_spec1 with "Htab").
-              iIntros (finish) "Hfinish". wp_pures.
+              destruct (decide (s2 = s1)); simplify_eq; last first.
 
-              case_bool_decide; wp_pures; simplify_eq.
-              + wp_bind (finish #()).
-                assert (c0 = 0); [lia|]. simplify_eq.
+              + wp_apply v_finish_spec1_bad; try done.
+                iIntros (finish) "Hfinish". wp_pures.
 
-                iApply ("Hfinish" $! s1 ⊤ tA' with "[//] [$Htok $Hser' $HA_un $hashs1]");
-                  first by iLeft.
-                iNext. iIntros ([]) "Htok"; wp_pures; last first.
-                { iApply ("HΦ" $! (None)). eauto. }
+                case_bool_decide; wp_pures; simplify_eq.
+                * wp_bind (finish #()).
+                  assert (c0 = 0); [lia|]. simplify_eq.
 
-                wp_apply gwp_list_tail; [done|].
-                iIntros (vl Hl).
+                  iApply ("Hfinish" $! _ _ ⊤ with "[//] [$Htok $Hserproph $Hser3 $hashs1 //]").
+                  iNext. iIntros ([]) "[Htok %]"; simplify_eq; wp_pures.
+                  iApply ("HΦ" $! (None)). by iFrame.
 
-                iMod (na_inv_acc with "Htab Htok") as "(Htabo & Htok & Hclose_tab)"; [solve_ndisj|solve_ndisj|].
-                iDestruct "Htabo" as (???) "(Hl & >%Hm & Hbigsep & Hfrag)".
-                wp_pures.
+                * iMod (na_inv_acc with "Htab Htok") as "(Htabo & Htok & Hclose_tab)"; [solve_ndisj|solve_ndisj|].
+                  iDestruct "Htabo" as (??) "(Hl & >%Hm & Hbigsep & Hge)". wp_load.
 
-                iPoseProof (idcntr_agree with "[$Hid $Hfrag]") as (->) "[Hid Hfrag]".
-                iMod (idcntr_update with "[$Hid $Hfrag]") as "[Hid Hfrag]".
+                  iDestruct "Hge" as "[Hpos'|[Hpos'|[Hpos' %Hge]]]";
+                    iPoseProof (pos_agree with "Hpos Hpos'") as (?) "[Hpos Hpos']"; 
+                    simplify_eq.
 
-                (* iPoseProof (idcntr_agree with "[$Hst $Hfrag]") as (->) "[Hst Hfrag]".
-                iMod (global_state_update_empty with "[$Hst $Hfrag]") as "[Hst Hfrag]". *)
-                
-                iMod ("Hclose_tab" with "[$Hl $Hbigsep $Htok $Hfrag]") as "Htok"; try done.
-                (* { iFrame "%". iPureIntro. intros ?. apply Hci. lia. } *)
-                
-                iApply ("HΦ" $! (Some _)).
+                  iMod (pos_update1 with "Hpos Hpos'") as "(Hpos & Hpos' & Hfrag)".
 
-                destruct (decide (s2 = s1)); simplify_eq;
-                  [iMod ("Hrel" $! ⊤ with "[//] Htok [Hserproph] Hser1 HA") as "[Htok #HA']";
-                    try by iRight|]; iFrame "# ∗ %"; iModIntro; repeat (iExists _); 
-                    iSplit; try (iSplit; try done; iPureIntro; repeat f_equal; lia);
-                    [iLeft|iRight]; iFrame "# ∗ %"; iExists _; iExists (c0+1);
+                  wp_bind (map.map_insert _ _ _). wp_pures.
+                  iApply (gwp_map_insert #cntr (#c0, finish)%V d m _ _); [done|done|].
+                  
+                  iModIntro. iIntros (d') "%Hmap'". wp_store.
+
+                  (* iMod (msize_update _ (s+1) with "[$Hms $Hs]") as "[Hms Hs]". *)
+                  wp_pures. wp_apply (gwp_list_tail with "[//]").
+                  iIntros "/=" (tl Htl). wp_pures.
+                  iMod ("Hclose_tab" with "[$Hl Hbigsep $Htok Hfinish Hpos' Hfrag]") as "Htok".
+                  { iNext. iFrame "%". iSplitR "Hpos'"; last first.
+                    { do 2 iRight. iFrame "∗". admit. }
+                    iApply (big_sepM_insert_2 with "[Hfinish Hfrag]"); last done.
+                    assert (c0 > 0).
+                    { apply Nat.neq_0_lt_0. intros ->. by apply H0. }
+                    repeat iExists _. repeat (try (iSplit; eauto)).
+                    iRight. iFrame. iExists _. iLeft. by iFrame "# ∗". }
+
+                  iModIntro. iApply ("HΦ" $! (Some _)). iFrame "∗ % #". 
+                  repeat (iExists _). iSplit.
+                  { iPureIntro. split; repeat f_equal. instantiate (1 := cntr + 1). lia. }
+                  iRight; iFrame "# ∗ %"; iExists _, (cntr+1);
+                    iSplit; iPureIntro; repeat f_equal; lia.
+                  
+              + wp_apply v_finish_spec1; try done.
+                iIntros (finish) "Hfinish". wp_pures.
+
+                case_bool_decide; wp_pures; simplify_eq.
+                * wp_bind (finish #()).
+                  assert (c0 = 0); [lia|]. simplify_eq.
+
+                  iApply ("Hfinish" $! _ _ ⊤ with "[//] [$Htok $Hserproph $Hser3 //]").
+                  iNext. iIntros ([]) "Htok"; simplify_eq; wp_pures; last first.
+                  { iApply ("HΦ" $! (None)). by iFrame. }
+
+                  wp_pures. wp_apply (gwp_list_tail with "[//]").
+                  iIntros "/=" (tl Htl). wp_pures.
+
+                  iApply ("HΦ" $! (Some _)).
+                  iMod ("Hrel" $! ⊤ with "[//] Htok [Hserproph] Hser1 HA") as "[Htok #HA']";
+                    try by iRight.
+                  iFrame "# ∗". iModIntro; repeat (iExists _);
+                  iSplit; try (iSplit; try done; iPureIntro; repeat f_equal; 
+                    instantiate (1 := cntr + 1); lia).
+                  iLeft. iFrame "# ∗ %"; iExists _, (cntr+1);
+                    iSplit; iPureIntro; repeat f_equal; lia.
+                    
+                * iMod (na_inv_acc with "Htab Htok") as "(Htabo & Htok & Hclose_tab)"; [solve_ndisj|solve_ndisj|].
+                  iDestruct "Htabo" as (??) "(Hl & >%Hm & Hbigsep & >Hge)". wp_load.
+
+                  iDestruct "Hge" as "[Hpos'|[Hpos'|[Hpos' %Hge]]]";
+                    iPoseProof (pos_agree with "Hpos Hpos'") as (?) "[Hpos Hpos']"; 
+                    simplify_eq.
+
+                  wp_bind (map.map_insert _ _ _). wp_pures.
+                  iApply (gwp_map_insert #cntr (#c0, finish)%V d m _ _); [done|done|].
+                  
+                  iModIntro. iIntros (d') "%Hmap'". wp_store.
+
+                  wp_pures. wp_apply (gwp_list_tail with "[//]").
+                  iIntros "/=" (tl Htl). wp_pures.
+                  iMod ("Hclose_tab" with "[$Hl Hbigsep $Htok Hfinish Hpos]") as "Htok".
+                  { iNext. iFrame "%". iSplitR "Hpos"; last first; try by iLeft.
+                    iApply (big_sepM_insert_2 with "[Hfinish]"); last done.
+                    assert (c0 > 0).
+                    { apply Nat.neq_0_lt_0. intros ->. by apply H0. }
+                    repeat iExists _. repeat (try (iSplit; eauto)).
+                    do 2 iLeft. iFrame. eauto. }
+
+                  iApply ("HΦ" $! (Some _)).
+                  iMod ("Hrel" $! ⊤ with "[//] Htok [Hserproph] Hser1 HA") as "[Htok #HA']";
+                    try by iRight.
+                  iFrame "# ∗"; iModIntro; repeat (iExists _).
+                  iSplit; try (iSplit; try done; iPureIntro; repeat f_equal; 
+                    instantiate (1 := cntr + 1); lia).
+                  iLeft. iFrame "# ∗ %"; iExists _, (cntr+1);
                     iSplit; iPureIntro; repeat f_equal; lia.
 
-              + iMod (na_inv_acc with "Htab Htok") as "(Htabo & Htok & Hclose_tab)"; [solve_ndisj|solve_ndisj|].
-                iDestruct "Htabo" as (???) "(Hl & >%Hm & Hbigsep & Hfrag)". wp_load.
+            - destruct (decide (s2 = s1)); simplify_eq; last first.
 
-                (* iPoseProof (idcntr_agree with "[$Hst $Hfrag]") as (->) "[Hst Hfrag]".
-                iPoseProof (msize_agree with "[$Hms $Hs]") as (<-) "[Hms Hs]".
-                iMod (global_state_update_singleton with "[$Hst $Hfrag]") as "(Hst & Hins & Hfrag)". *)
-                iPoseProof (idcntr_agree with "[$Hid $Hfrag]") as (->) "[Hid Hfrag]".
-                iMod (idcntr_update with "[$Hid $Hfrag]") as "[Hid Hfrag]".
+              + wp_apply v_finish_spec2_bad; try done.
+                iIntros (finish) "Hfinish". wp_pures.
 
-                (* assert (m0 !! #c1 = None). { apply Hci. lia. } *)
-                wp_bind (map.map_insert _ _ _). wp_pures.
-                iApply (gwp_map_insert #c1 (#c0, finish)%V d m _ _); [done|done|].
+                case_bool_decide; wp_pures; simplify_eq.
+                * wp_bind (finish #()).
+                  assert (c0 = 0); [lia|]. simplify_eq.
+
+                  iApply ("Hfinish" $! _ _ _ ⊤ with "[//] [$Htok $Hserproph $Hser3 $hashs1 $Hinv //]").
+                  iNext. iIntros ([]) "[Htok %]"; simplify_eq; wp_pures.
+                  iApply ("HΦ" $! (None)). by iFrame.
                 
-                iModIntro. iIntros (d') "%Hmap'". wp_store.
-                (* iMod (msize_update _ (s+1) with "[$Hms $Hs]") as "[Hms Hs]". *)
-                wp_pures. wp_apply (gwp_list_tail with "[//]").
-                iIntros "/=" (tl Htl). wp_pures.
-                iMod ("Hclose_tab" with "[$Hl Hbigsep $Htok $Hfrag Hfinish]") as "Htok".
-                { iNext. iFrame "%".
-                  iApply (big_sepM_insert_2 with "[Hfinish]"); last done.
-                  iFrame "∗ #". iExists _.
-                  assert (c0 > 0).
-                  { apply Nat.neq_0_lt_0. intros ->. by apply H0. }
-                  do 2 iExists _. repeat (try (iSplit; eauto)).  }
+                * iMod (na_inv_acc with "Htab Htok") as "(Htabo & Htok & Hclose_tab)"; [solve_ndisj|solve_ndisj|].
+                  iDestruct "Htabo" as (??) "(Hl & >%Hm & Hbigsep & Hge)". wp_load.
 
-                iApply ("HΦ" $! (Some _)).
-                destruct (decide (s2 = s1)); simplify_eq;
-                  [iMod ("Hrel" $! ⊤ with "[//] Htok [Hserproph] Hser1 HA") as "[Htok #HA']";
-                    try by iRight|]; iFrame "# ∗ %"; iModIntro; repeat (iExists _);
-                    iSplit; try (iSplit; try done; iPureIntro; repeat f_equal; lia);
-                    [iLeft|iRight]; iFrame "# ∗ %"; iExists _; iExists (c1+1);
+                  iDestruct "Hge" as "[Hpos'|[Hpos'|[Hpos' %Hge]]]";
+                    iPoseProof (pos_agree with "Hpos Hpos'") as (?) "[Hpos Hpos']"; 
+                    simplify_eq.
+
+                  iMod (pos_update1 with "Hpos Hpos'") as "(Hpos & Hpos' & Hfrag)".
+
+                  wp_bind (map.map_insert _ _ _). wp_pures.
+                  iApply (gwp_map_insert #cntr (#c0, finish)%V d m _ _); [done|done|].
+                  
+                  iModIntro. iIntros (d') "%Hmap'". wp_store.
+
+                  (* iMod (msize_update _ (s+1) with "[$Hms $Hs]") as "[Hms Hs]". *)
+                  wp_pures. wp_apply (gwp_list_tail with "[//]").
+                  iIntros "/=" (tl Htl). wp_pures.
+                  iMod ("Hclose_tab" with "[$Hl Hbigsep $Htok Hfinish Hpos' Hfrag]") as "Htok".
+                  { iNext. iFrame "%". iSplitR "Hpos'"; last first.
+                    { do 2 iRight. iFrame "∗". admit. }
+                    iApply (big_sepM_insert_2 with "[Hfinish Hfrag]"); last done.
+                    assert (c0 > 0).
+                    { apply Nat.neq_0_lt_0. intros ->. by apply H0. }
+                    repeat iExists _. repeat (try (iSplit; eauto)).
+                    iRight. iFrame. iExists _. iRight. by iFrame "# ∗". }
+
+                  iModIntro. iApply ("HΦ" $! (Some _)). iFrame "∗ % #". 
+                  repeat (iExists _). iSplit.
+                  { iPureIntro. split; repeat f_equal. instantiate (1 := cntr + 1). lia. }
+                  iRight; iFrame "# ∗ %"; iExists _, (cntr+1);
                     iSplit; iPureIntro; repeat f_equal; lia.
 
-            - wp_apply (v_finish_spec2 with "Htab").
-              iIntros (finish) "Hfinish". wp_pures.
+              + wp_apply (v_finish_spec2 with "Htab").
+                iIntros (finish) "Hfinish". wp_pures.
 
-              case_bool_decide; wp_pures; simplify_eq.
-              * wp_bind (finish #()).
-                assert (c0 = 0); [lia|]. simplify_eq.
+                case_bool_decide; wp_pures; simplify_eq.
+                * wp_bind (finish #()).
+                  assert (c0 = 0); [lia|]. simplify_eq.
 
-                iApply ("Hfinish" $! _ ⊤ tA' with "[//] [$Htok $Hser' $HA_un $Hinv //]").
-                iNext. iIntros ([]) "Htok"; wp_pures; last first.
-                { iApply ("HΦ" $! (None)). eauto. }
+                  iApply ("Hfinish" $! _ _ ⊤ with "[//] [$Htok $Hserproph $Hser3 $Hinv $Hpos]"); eauto.
+                  iNext. iIntros ([]) "[Htok Hpos]"; wp_pures; last first.
+                  { iApply ("HΦ" $! (None)). eauto. }
 
-                wp_apply gwp_list_tail; [done|].
-                iIntros (vl Hl).
+                  wp_apply gwp_list_tail; [done|].
+                  iIntros (vl Hl). wp_pures.
+                  
+                  iApply ("HΦ" $! (Some _)).
 
-                iMod (na_inv_acc with "Htab Htok") as "(Htabo & Htok & Hclose_tab)"; [solve_ndisj|solve_ndisj|].
-                iDestruct "Htabo" as (???) "(Hl & >%Hm & Hbigsep & Hfrag)".
-                wp_pures.
-
-                iPoseProof (idcntr_agree with "[$Hid $Hfrag]") as (->) "[Hid Hfrag]".
-                iMod (idcntr_update with "[$Hid $Hfrag]") as "[Hid Hfrag]".
-
-                (* iPoseProof (idcntr_agree with "[$Hst $Hfrag]") as (->) "[Hst Hfrag]".
-                iMod (global_state_update_empty with "[$Hst $Hfrag]") as "[Hst Hfrag]". *)
-                
-                iMod ("Hclose_tab" with "[$Hl $Hbigsep $Htok $Hfrag]") as "Htok"; try done.
-                (* { iFrame "%". iIntros (id). iPureIntro. intros ?. apply Hci. lia. } *)
-                
-                iApply ("HΦ" $! (Some _)).
-
-                destruct (decide (s2 = s1)); simplify_eq;
-                  [iMod ("Hrel" $! ⊤ with "[//] Htok [Hserproph] Hser1 HA") as "[Htok #HA']";
-                    try by iRight|]; iFrame "# ∗ %"; iModIntro; repeat (iExists _); 
-                    iSplit; try (iSplit; try done; iPureIntro; repeat f_equal; lia);
-                    [iLeft|iRight]; iFrame "# ∗ %"; iExists _; iExists (c0+1);
+                  iMod ("Hrel" $! ⊤ with "[//] Htok [Hserproph] Hser1 HA") as "[Htok #HA']";
+                    try by iRight.
+                  iFrame "# ∗"; iModIntro; repeat (iExists _).
+                  iSplit; try (iSplit; try done; iPureIntro; repeat f_equal; 
+                    instantiate (1 := cntr + 1); lia).
+                  iLeft. iFrame "# ∗ %". iExists _, (cntr+1);
                     iSplit; iPureIntro; repeat f_equal; lia.
-              
-              * iMod (na_inv_acc with "Htab Htok") as "(Htabo & Htok & Hclose_tab)"; [solve_ndisj|solve_ndisj|].
-                iDestruct "Htabo" as (???) "(Hl & >%Hm & Hbigsep & Hfrag)". wp_load.
-
-                (* iPoseProof (idcntr_agree with "[$Hst $Hfrag]") as (->) "[Hst Hfrag]".
-                iPoseProof (msize_agree with "[$Hms $Hs]") as (<-) "[Hms Hs]".
-                iMod (global_state_update_singleton with "[$Hst $Hfrag]") as "(Hst & Hins & Hfrag)". *)
-                iPoseProof (idcntr_agree with "[$Hid $Hfrag]") as (->) "[Hid Hfrag]".
-                iMod (idcntr_update with "[$Hid $Hfrag]") as "[Hid Hfrag]".
-
-                (* assert (m0 !! #c1 = None). { apply Hci. lia. } *)
-                wp_bind (map.map_insert _ _ _). wp_pures.
-                iApply (gwp_map_insert #c1 (#c0, finish)%V d m _ _); [done|done|].
                 
-                iModIntro. iIntros (d') "%Hmap'". wp_store.
-                (* iMod (msize_update _ (s+1) with "[$Hms $Hs]") as "[Hms Hs]". *)
-                wp_pures. wp_apply (gwp_list_tail with "[//]").
-                iIntros "/=" (tl Htl). wp_pures.
-                iMod ("Hclose_tab" with "[$Hl Hbigsep $Htok $Hfrag Hfinish]") as "Htok".
-                { iNext. iFrame "%".
-                  iApply (big_sepM_insert_2 with "[Hfinish]"); last done.
-                  iFrame "∗ #". iExists _.
-                  assert (c0 > 0).
-                  { apply Nat.neq_0_lt_0. intros ->. by apply H0. }
-                  do 2 iExists _. repeat (try (iSplit; eauto)). }
+                * iMod (na_inv_acc with "Htab Htok") as "(Htabo & Htok & Hclose_tab)"; [solve_ndisj|solve_ndisj|].
+                  iDestruct "Htabo" as (??) "(Hl & >%Hm & Hbigsep & >Hge)". wp_load.
 
-                iApply ("HΦ" $! (Some _)).
-                destruct (decide (s2 = s1)); simplify_eq;
-                  [iMod ("Hrel" $! ⊤ with "[//] Htok [Hserproph] Hser1 HA") as "[Htok #HA']";
-                    try by iRight|]; iFrame "# ∗ %"; iModIntro; repeat (iExists _);
-                    iSplit; try (iSplit; try done; iPureIntro; repeat f_equal; lia);
-                    [iLeft|iRight]; iFrame "# ∗ %"; iExists _; iExists (c1+1);
+                  iDestruct "Hge" as "[Hpos'|[Hpos'|[Hpos' %Hge]]]";
+                    iPoseProof (pos_agree with "Hpos Hpos'") as (?) "[Hpos Hpos']"; 
+                    simplify_eq.
+
+                  wp_bind (map.map_insert _ _ _). wp_pures.
+                  iApply (gwp_map_insert #cntr (#c0, finish)%V d m _ _); [done|done|].
+                  
+                  iModIntro. iIntros (d') "%Hmap'". wp_store.
+
+                  wp_pures. wp_apply (gwp_list_tail with "[//]").
+                  iIntros "/=" (tl Htl). wp_pures.
+                  iMod ("Hclose_tab" with "[$Hl Hbigsep $Htok Hfinish Hpos]") as "Htok".
+                  { iNext. iFrame "%". iSplitR "Hpos"; last first; try by iLeft.
+                    iApply (big_sepM_insert_2 with "[Hfinish]"); last done.
+                    assert (c0 > 0).
+                    { apply Nat.neq_0_lt_0. intros ->. by apply H0. }
+                    repeat iExists _. repeat (try (iSplit; [done|])).
+                    iLeft. iRight. by iFrame "# ∗". }
+
+                  iApply ("HΦ" $! (Some _)).
+
+                  iMod ("Hrel" $! ⊤ with "[//] Htok [Hserproph] Hser1 HA") as "[Htok #HA']";
+                    try by iRight.
+                  iFrame "# ∗"; iModIntro; repeat (iExists _).
+                  iSplit; try (iSplit; try done; iPureIntro; repeat f_equal; 
+                      instantiate (1 := cntr + 1); lia);
+                  iLeft; iFrame "# ∗ %"; iExists _, (cntr+1);
                     iSplit; iPureIntro; repeat f_equal; lia. }
               
-          { iIntros (???) "!# (Htok & Hproof & Hid) HΦ".
-            wp_pures. i_pures. iDestruct "Hproof" as (? -> ) "Hproof".
-            wp_pures. iDestruct "Hproof" as "(% & %)".
-            wp_apply gwp_list_head; [done| ].
-            iIntros (vl [[-> ->] | (s1' &?& -> & -> )]).
-            { wp_pures. iModIntro.
-              iApply ("HΦ" $! None). iFrame. }
+          { iApply (refines_un_auth_unauth with "Htab Hser' Hser3 Hcount Hdeser Hauth_un"). } }
+        { rewrite interp_un_arr_unfold.
+          iIntros (w) "!# #Hauth Htok /=".
+          interp_unfold in "Hevi Hauth".
+          rewrite interp_var3_ext4.
+          iDestruct "Hauth" as "[(% & % & Hauth_un)|->]"; wp_pures; last first.
+          { iFrame. iModIntro.
+            interp_unfold!. rewrite interp_var2_ext3.
+            iIntros (???) "!# (Htok & Hproof & Hpos) HΦ".
+            wp_pures. iApply ("HΦ" $! None). by iFrame. }
 
-            wp_pures. wp_apply "Hdeser"; [done|].
-            iIntros (?) "Hdepar".
-            wp_apply "Hdepar"; [done|].
-            iIntros ([]); last first.
-            { iIntros "_". wp_pures. iApply ("HΦ" $! None). iFrame. eauto. }
+          iDestruct "Hevi" as "[Hrel Hevi_un]".    
+          iDestruct "Hevi_un" as (tA' ??? ->) "(#Hser' & #Hser3 & #Hcount & #Hdeser)".
+          simplify_eq.
+          iFrame. iModIntro. interp_unfold!.
+          rewrite interp_var2_ext3.
+          iApply (refines_un_auth_unauth with "Htab Hser' Hser3 Hcount Hdeser Hauth_un"). } }
+      { rewrite interp_un_arr_unfold.
+        iIntros (?) "!# #Hevi Htok".
+        wp_pures. iModIntro. iFrame. clear.
+        rewrite interp_un_arr_unfold.
+        iIntros (w) "!# #Hauth Htok /=".
+        interp_unfold in "Hevi Hauth".
+        rewrite interp_var3_ext4.
+        iDestruct "Hauth" as "[(% & % & Hauth_un)|->]"; wp_pures; last first.
+        { iFrame. iModIntro.
+          interp_unfold!. rewrite interp_var2_ext3.
+          iIntros (???) "!# (Htok & Hproof & Hpos) HΦ".
+          wp_pures. iApply ("HΦ" $! None). by iFrame. }
             
-            iPoseProof "Hauth_un" as "[(%&%)|(%&%&%&#Hinv)]";
-              simplify_eq; iIntros "[Hserser Hserproph]";
-              iPoseProof ("Hserproph" with "Hserser") as ">[#HA_un [%s2 #Hserproph]]";
-              wp_pures; wp_apply ("Hcount" $! _ _ ⊤ with "[//] [$Hserproph $Htok]");
-              iIntros (?) "[_ Htok]"; wp_pures.
-            - 
-
-          }
-        }
-      }
-    }
-      
-            
+        iDestruct "Hevi" as (tA' ??? ->) "(#Hser' & #Hser3 & #Hcount & #Hdeser)".
+        simplify_eq.
+        iFrame. iModIntro. interp_unfold!.
+        rewrite interp_var2_ext3.
+        iApply (refines_un_auth_unauth with "Htab Hser' Hser3 Hcount Hdeser Hauth_un"). } }
+    { rewrite interp_un_forall_unfold.
+      iIntros (A v) "!# _ Htok".
+      wp_pures.
+      iModIntro. iFrame. clear.
+      rewrite interp_un_arr_unfold.
+      iIntros (?) "!# #Hevi Htok".
+      wp_pures. iModIntro. iFrame. clear.
+      rewrite interp_un_arr_unfold.
+      iIntros (w) "!# #Hauth Htok /=".
+      interp_unfold in "Hevi Hauth".
+      rewrite interp_var3_ext4.
+      iDestruct "Hauth" as "[(% & % & Hauth_un)|->]"; wp_pures; last first.
+      { iFrame. iModIntro.
+        interp_unfold!. rewrite interp_var2_ext3.
+        iIntros (???) "!# (Htok & Hproof & Hpos) HΦ".
+        wp_pures. iApply ("HΦ" $! None). by iFrame. }
+          
+      iDestruct "Hevi" as (tA' ??? ->) "(#Hser' & #Hser3 & #Hcount & #Hdeser)".
+      simplify_eq.
+      iFrame. iModIntro. interp_unfold!.
+      rewrite interp_var2_ext3.
+      iApply (refines_un_auth_unauth with "Htab Hser' Hser3 Hcount Hdeser Hauth_un"). }
   Admitted.
-
+  
   Lemma refines_Authenticatable Θ (Δ : ctxO Σ Θ) :
     ⊢ REL v_Authenticable << i_Authenticable : ⟦ Authenticatable ⟧ (auth_ctx Δ).
   Proof.
@@ -1102,16 +1562,12 @@ Section proof.
     wp_apply gwp_map_empty; [done|].
     iIntros (d) "Hd". wp_alloc l as "Hl". wp_pures.
     
-    iMod msize_alloc as (γm) "[Hmfrag Hmauth]".
-    iMod idcntr_alloc as (γc) "[Hcauth Hcfrag]".
+    iMod pos_alloc as (γm) "[Hpos Hpos']".
     
-    iMod (na_inv_alloc seqG_name ⊤ tableN (is_susp_table l) with "[$Hd $Hl Hmauth Hcauth]") as "#Htab".
-    { iNext. iExists 0.
-      rewrite /msize_auth /idcntr_frag. iFrame.
-      iSplitR; [by iApply big_sepM_empty|].
-      iSplitL "Hmauth"; [admit|].
-      iSplitL "Hcauth"; [admit|].
-      iIntros (id). done. }
+    iMod (na_inv_alloc seqG_name ⊤ tableN (is_susp_table l) with "[$Hd $Hl Hpos']") as "#Htab".
+    { iNext. iSplitR; last first.
+      { iLeft. admit. } 
+      by iApply big_sepM_empty. }
     
     iAssert (|={⊤}=> spec_ideal tᵢ (fill Kᵢ (i_Auth_auth, i_Auth_mu, i_Auth_pair, i_Auth_sum, i_Auth_string, i_Auth_int, i_auth, i_unauth)))%I with "[Hi]" as ">Hi"; [admit|].
     
@@ -1120,52 +1576,130 @@ Section proof.
     i_bind (i_unauth).    
     iPoseProof (refines_auth_unauth with "Htab [$Hi $Htok]") as "Hwp".
     wp_apply (wp_wand with "Hwp").
-    iIntros (?) "(% & Hi & #Hauth & Htok)".
+    iIntros (?) "(% & Hi & #[Hauth Hauth_un] & Htok)".
     iSimpl in "Hi".
     i_pures. wp_pures.
     iModIntro. iFrame.
     rewrite /Authenticatable.
-    interp_unfold!.
-    iExists (lrel_evidence authBaseN).
-    interp_unfold.
-    iExists  _, _, _, _.
-    do 2 (iSplit; [done|]).
-    iSplit; [|done].
-    interp_unfold.
-    iExists _, _, _, _.
-    do 2 (iSplit; [done|]).
-    iSplit; last first.
-    { iApply refines_auth_auth. }
-    interp_unfold.
-    iExists _, _, _, _.
-    do 2 (iSplit; [done|]).
-    iSplit; last first.
-    { interp_unfold!. iApply refines_Auth_int. }
-    interp_unfold!.
-    iExists _, _, _, _.
-    do 2 (iSplit; [done|]).
-    iSplit; last first.
-    { interp_unfold!. iApply refines_Auth_string. }
-    interp_unfold!.
-    iExists _, _, _, _.
-    do 2 (iSplit; [done|]).
-    iSplit; last first.
-    { iApply refines_Auth_sum. }
-    interp_unfold!.
-    iExists _, _, _, _.
-    do 2 (iSplit; [done|]).
-    iSplit; last first.
-    { iApply refines_Auth_pair. }
-    interp_unfold.
-    iExists _, _, _, _.
-    do 2 (iSplit; [done|]).
-    iSplit; last first.
-    { iApply refines_Auth_mu. }
-    iApply refines_Auth_auth.
+    iSplit; interp_unfold!.
+    { iExists lrel_evidence.
+      iSplit; interp_unfold!.
+      { iExists  _, _, _, _.
+        do 2 (iSplit; [done|]).
+        iSplit; [|done].
+        interp_unfold.
+        iExists _, _, _, _.
+        do 2 (iSplit; [done|]).
+        iSplit; last first.
+        { iPoseProof refines_auth_auth as "[$ _]". }
+        interp_unfold.
+        iExists _, _, _, _.
+        do 2 (iSplit; [done|]).
+        iSplit; last first.
+        { interp_unfold!. iPoseProof (refines_Auth_int authBaseN) as "[Hint _]".
+          rewrite /lrel_car /=. rewrite interp_unseal //. }
+        interp_unfold!.
+        iExists _, _, _, _.
+        do 2 (iSplit; [done|]).
+        iSplit; last first.
+        { interp_unfold!. iPoseProof (refines_Auth_string authBaseN) as "[Hstr _]".
+          rewrite /lrel_car /=. rewrite interp_unseal //. }
+        interp_unfold!.
+        iExists _, _, _, _.
+        do 2 (iSplit; [done|]).
+        iSplit; last first.
+        { iPoseProof refines_Auth_sum as "[$ _]". }
+        interp_unfold!.
+        iExists _, _, _, _.
+        do 2 (iSplit; [done|]).
+        iSplit; last first.
+        { iPoseProof refines_Auth_pair as "[$ _]". }
+        interp_unfold.
+        iExists _, _, _, _.
+        do 2 (iSplit; [done|]).
+        iSplit; last first.
+        { iPoseProof refines_Auth_mu as "[$ _]". }
+        iPoseProof refines_Auth_auth as "[$ _]". }
+      { rewrite interp_un_prod_unfold.
+        iExists _, _.
+        iSplit; try done.
+        rewrite interp_un_prod_unfold.
+        iSplit; try done.
+        iExists _, _.
+        iSplit; try done.
+        iSplit; last first.
+        { iPoseProof refines_auth_auth as "[_ $]". }
+        rewrite interp_un_prod_unfold.
+        iExists _, _.
+        iSplit; try done.
+        iSplit; last first.
+        { interp_unfold!. iPoseProof (refines_Auth_int authBaseN) as "[_ Hint]".
+          rewrite /lrel_car /=. rewrite interp_unseal //. }
+        rewrite interp_un_prod_unfold.
+        iExists _, _.
+        iSplit; try done.
+        iSplit; last first.
+        { interp_unfold!. iPoseProof (refines_Auth_string authBaseN) as "[_ Hstr]".
+          rewrite /lrel_car /=. rewrite interp_unseal //. }
+        rewrite interp_un_prod_unfold.
+        iExists _, _.
+        iSplit; try done.
+        iSplit; last first.
+        { iPoseProof refines_Auth_sum as "[_ $]". }
+        rewrite interp_un_prod_unfold.
+        iExists _, _.
+        iSplit; try done.
+        iSplit; last first.
+        { iPoseProof refines_Auth_pair as "[_ $]". }
+        rewrite interp_un_prod_unfold.
+        iExists _, _.
+        iSplit; try done.
+        iSplit; last first.
+        { iPoseProof refines_Auth_mu as "[_ $]". }
+        iPoseProof refines_Auth_auth as "[_ $]". } }
+    { rewrite interp_un_exists_unfold.
+      iExists lrel_evidence.
+      rewrite interp_un_prod_unfold.
+      iExists _, _.
+      iSplit; try done.
+      rewrite interp_un_prod_unfold.
+      iSplit; try done.
+      iExists _, _.
+      iSplit; try done.
+      iSplit; last first.
+      { iPoseProof refines_auth_auth as "[_ $]". }
+      rewrite interp_un_prod_unfold.
+      iExists _, _.
+      iSplit; try done.
+      iSplit; last first.
+      { interp_unfold!. iPoseProof (refines_Auth_int authBaseN) as "[_ Hint]".
+        rewrite /lrel_car /=. rewrite interp_unseal //. }
+      rewrite interp_un_prod_unfold.
+      iExists _, _.
+      iSplit; try done.
+      iSplit; last first.
+      { interp_unfold!. iPoseProof (refines_Auth_string authBaseN) as "[_ Hstr]".
+        rewrite /lrel_car /=. rewrite interp_unseal //. }
+      rewrite interp_un_prod_unfold.
+      iExists _, _.
+      iSplit; try done.
+      iSplit; last first.
+      { iPoseProof refines_Auth_sum as "[_ $]". }
+      rewrite interp_un_prod_unfold.
+      iExists _, _.
+      iSplit; try done.
+      iSplit; last first.
+      { iPoseProof refines_Auth_pair as "[_ $]". }
+      rewrite interp_un_prod_unfold.
+      iExists _, _.
+      iSplit; try done.
+      iSplit; last first.
+      { iPoseProof refines_Auth_mu as "[_ $]". }
+      iPoseProof refines_Auth_auth as "[_ $]". }
   Admitted.
 
   Lemma refines_authentikit_func Θ (Δ : ctxO Σ Θ) :
-    ⊢ REL v_Authentikit << i_Authentikit : ⟦ Authentikit_func var2 var1 var0 ⟧ (auth_ctx Δ).
+    ⊢ REL v_Authentikit << i_Authentikit : ⟦ Authentikit_func var1 var0 ⟧ (auth_ctx Δ).
   Proof.
     iIntros (??) "[Hi Htok]".
     rewrite /i_Authentikit /v_Authentikit.
@@ -1174,20 +1708,30 @@ Section proof.
     i_bind (i_Authenticable).
     iPoseProof (refines_Authenticatable with "[$Hi $Htok]") as "H".
     wp_apply (wp_wand with "H").
-    iIntros (?) "(% & Hv & #Hauth & Htok)".
+    iIntros (?) "(% & Hv & #[Hauth Hauth_un] & Htok)".
     iSimpl in "Hv".
     i_pures. wp_pures.
     iModIntro. iFrame.
     rewrite interp_unseal -/interp.interp_def.
-    iExists _, _, _, _; rewrite -!/interp.interp_def.
-    do 2 (iSplit; [done|]).
-    iSplit; [|done].
-    iExists _, _, _, _; rewrite -!/interp.interp_def.
-    do 2 (iSplit; [done|]).
     iSplit.
-    { iPoseProof refines_auth_return as "H". rewrite interp_unseal //. }
-    iPoseProof refines_auth_bind as "?".
-    rewrite interp_unseal //.
+    { iExists _, _, _, _; rewrite -!/interp.interp_def.
+      do 2 (iSplit; [done|]).
+      iSplit; [|done].
+      iExists _, _, _, _; rewrite -!/interp.interp_def.
+      do 2 (iSplit; [done|]).
+      iSplit.
+      { iPoseProof refines_auth_return as "[H _]". rewrite interp_unseal //. }
+      iPoseProof refines_auth_bind as "[? _]".
+      rewrite interp_unseal //. }
+    { iExists _, _; rewrite -!/interp.interp_def.
+      iSplit; [done|].
+      iSplit; [|done].
+      iExists _, _; rewrite -!/interp.interp_def.
+      iSplit; [done|].
+      iSplit.
+      { iPoseProof refines_auth_return as "[_ H]". rewrite interp_unseal //. }
+      iPoseProof refines_auth_bind as "[_ ?]".
+      rewrite interp_unseal //. }
   Admitted.
 
   Lemma refines_authentikit Θ (Δ : ctxO Σ Θ) :
@@ -1196,9 +1740,15 @@ Section proof.
     iIntros (??) "Hi".
     iPoseProof (refines_authentikit_func with "Hi") as "H".
     wp_apply (wp_wand  with "H").
-    iIntros (?) "(% & $ & #Hauth & Htok)".
-    do 3 setoid_rewrite interp_exists_unfold. iFrame.
-    by iExists lrel_hash_fail_option, lrel_auth, lrel_auth_comp.
+    iIntros (?) "(% & $ & #Hauth & $)".
+    iPoseProof "Hauth" as "[Hauth' Hauth_un]".
+    iSplit.
+    - rewrite interp_exists_unfold. iExists lrel_auth.
+      iSplit.
+      + rewrite interp_exists_unfold. by iExists lrel_auth_comp.
+      + rewrite interp_un_exists_unfold. by iExists lrel_auth_comp.
+    - do 2 setoid_rewrite interp_un_exists_unfold. 
+      by iExists lrel_auth, lrel_auth_comp.
   Qed.
 
   Lemma refines_run w (c1 c2 : expr) A :
@@ -1212,62 +1762,57 @@ Section proof.
     wp_bind c1; i_bind c2.
     iSpecialize ("Hc" with "[$Hi $Htok]").
     wp_apply (wp_wand with "Hc").
-    iIntros (f1) "(%f2 & Hi & Hc & Htok) /=".
+    iIntros (f1) "(%f2 & Hi & [Hc Hc_un] & Htok) /=".
     rewrite /v_Authenticable_run.
     rewrite /i_Authenticable /v_Authenticable /v_Authenticable_run.
     wp_apply gwp_map_empty; [done|].
     iIntros (d) "Hd". wp_alloc l as "Hl". wp_pures.
     
-    iMod msize_alloc as (γm) "[Hmfrag Hmauth]".
-    iMod idcntr_alloc as (γc) "[Hcauth Hcfrag]".
+    iMod pos_alloc as (γm) "[Hpos Hpos']".
     
-    iMod (na_inv_alloc seqG_name ⊤ tableN (is_susp_table l) with "[$Hd $Hl Hmauth Hcauth]") as "#Htab".
-    { iNext. iExists 0.
-      rewrite /msize_auth /idcntr_frag. iFrame.
-      iSplitR; [by iApply big_sepM_empty|].
-      iSplitL "Hmauth"; [admit|].
-      iSplitL "Hcauth"; [admit|].
-      iIntros (id). done. }
+    iMod (na_inv_alloc seqG_name ⊤ tableN (is_susp_table l) with "[$Hd $Hl Hpos']") as "#Htab".
+    { iNext. iSplitR; last admit.
+      by iApply big_sepM_empty. }
 
     wp_rec. wp_pures.
     wp_rec. wp_pures.    
     wp_pures; i_pures.
-    iMod (init_global_state with "[Hcfrag]") as "Hst"; [admit|].
-    wp_apply ("Hc" with "[$Hi $Htok $Hprf Hmfrag Hst]").
-    { instantiate (4 := 0). iSplit. { iPureIntro. f_equal. }
-      rewrite /msize_frag. iFrame. admit. }
+
+    wp_apply ("Hc" with "[$Hi $Htok $Hprf Hpos]").
+    { instantiate (1 := 0). iSplit. { iPureIntro. f_equal. }
+      admit. }
 
     iIntros (?) "(Htok & Ho)".
     destruct o1; last first.
     { wp_pures. iExists None. by iFrame. }
     
     iMod (na_inv_acc with "Htab Htok") as "(Htabo & Htok & Hclose_tab)"; [solve_ndisj|solve_ndisj|].
-    iDestruct "Htabo" as (????) "(Hl & >%Hm & Hbigsep & >Hmauth & Hfrag & >%Hci)".
-    iDestruct "Ho" as (????????) "(Hi & % & Hst & Hmfrag & Hpost)".
-    iPoseProof (msize_agree with "[$Hmauth $Hmfrag]") as (->) "[Hmauth Hmfrag]".
+    iDestruct "Htabo" as (??) "(Hl & >%Hm & Hbigsep & >Hge)".
     wp_pures. wp_load.
     wp_bind (map.map_is_empty _).
     iApply (gwp_map_is_empty with "[]"); [done|].
     iModIntro. iIntros (?) "%".
-    simpl in H0. subst.
-    iDestruct "Hpost" as "[[-> Hpost]|[% Hpost]]".
-    - wp_pures.
-      destruct! H. simplify_eq. wp_pures.
-      iMod ("Hclose_tab" with "[$Htok $Hbigsep $Hmauth $Hfrag $Hl]") as "Htok".
-      { iNext. iFrame "%". }
-      iModIntro. iExists (Some _).
-      iDestruct "Hpost" as (???) "(% & Hprf' & #HA)".
-      iFrame "∗". iSplit; first done. by simplify_eq.
-    - destruct l2; [done|]. wp_pures.
-      iMod ("Hclose_tab" with "[$Htok $Hbigsep $Hmauth $Hfrag $Hl]") as "Htok".
-      { iNext. iFrame "%". }
+    simpl in H. subst.
+    iDestruct "Ho" as (????[??]) "[(% & Hi & Hpost & Hpos)|(Hpost & Hpos)]"; simplify_eq;
+      iDestruct "Hge" as "[Hpos'|[Hpos'|[Hpos' %Hge]]]";
+      iPoseProof (pos_agree with "Hpos Hpos'") as (?) "[Hpos Hpos']"; 
+      simplify_eq.
+    - destruct (map.map_length m); wp_pures;
+      iMod ("Hclose_tab" with "[$Hl $Htok $Hbigsep Hpos']") as "Htok";
+        try (iNext; iFrame "%"; by iLeft);
+      iModIntro; [iExists (Some _)|iExists None]; iSplit; eauto.
+      iDestruct "Hpost" as (???) "(% & Hprf' & #HA)". simplify_eq.
+      iFrame "∗ #".
+    - destruct (map.map_length m) as [|n'] eqn:Hn; try lia. wp_pures.
+      iMod ("Hclose_tab" with "[$Hl $Htok $Hbigsep Hpos']") as "Htok".
+      { iNext. iFrame "%". iRight. iRight. iFrame. iPureIntro. lia. }
       iModIntro. iExists None. by iFrame.
   Admitted.
 
   Lemma refines_instantiate (c1 c2 : expr) (τ : type _ ⋆) :
-    (REL c1 << c2 : ⟦ ∀: ⋆ ⇒ ⋆; ⋆ ⇒ ⋆; ⋆ ⇒ ⋆, Authentikit_func var2 var1 var0 → var0 τ ⟧ ∅) -∗
-    REL c1 #~ #~ #~ v_Authentikit
-     << c2 #~ #~ #~ i_Authentikit : lrel_auth_comp (⟦ τ ⟧ (auth_ctx ∅)).
+    (REL c1 << c2 : ⟦ ∀: ⋆ ⇒ ⋆; ⋆ ⇒ ⋆, Authentikit_func var1 var0 → var0 τ ⟧ ∅) -∗
+    REL c1 #~ #~ v_Authentikit
+     << c2 #~ #~ i_Authentikit : lrel_auth_comp (⟦ τ ⟧ (auth_ctx ∅)).
   Proof.
     iIntros "Hc" (??) "[Hi Htok]".
     wp_bind v_Authentikit. i_bind i_Authentikit.
@@ -1278,13 +1823,8 @@ Section proof.
     iSpecialize ("Hc" with "[$Hi $Htok]").
     wp_apply (wp_wand with "Hc").
     iIntros (v1) "(%v2 & Hi & Hcnt & Htok)".
-    iSpecialize ("Hcnt" $! lrel_hash_fail_option with "[//]").
-    i_bind (v2 _).
-    iSpecialize ("Hcnt" with "[$Hi $Htok]").
-    wp_apply (wp_wand with "Hcnt").
-    iIntros (v1') "(%v2' & Hi & Hcnt & Htok)".
     iSpecialize ("Hcnt" $! lrel_auth with "[//]").
-    i_bind (v2' _).
+    i_bind (v2 _).
     iSpecialize ("Hcnt" with "[$Hi $Htok]").
     wp_apply (wp_wand with "Hcnt").
     iIntros (v1'') "(%v2'' & Hi & Hcnt & Htok)".
@@ -1292,7 +1832,7 @@ Section proof.
     i_bind (v2'' _).
     iSpecialize ("Hcnt" with "[$Hi $Htok]").
     wp_apply (wp_wand with "Hcnt").
-    iIntros (v1''') "(%v2''' & Hi & Hcnt & Htok)".
+    iIntros (v1''') "(%v2''' & Hi & [Hcnt _] & Htok)".
     i_bind (v2''' _).
     interp_unfold! in "Hcnt".
     iSpecialize ("Hcnt" with "[] [$Hi $Htok]"); rewrite -!/interp; [done|].
@@ -1305,10 +1845,10 @@ Section proof.
 
 End proof.
   
-Theorem authentikit_security Σ `{msizeG Σ, idcntrG Σ, stateG Σ, authPreG Σ, seqG Σ} (A : ∀ `{msizeG Σ, idcntrG Σ, stateG Σ, authG Σ, seqG Σ}, lrel Σ)
+Theorem authentikit_security Σ `{authPreG Σ, na_invG Σ, inG Σ poisonOSR} (A : ∀ `{authG Σ, seqG Σ, poisonOSG Σ}, (kindO Σ ⋆) )
   (φ : val → val → Prop) (cᵥ cᵢ : expr) (σ : state) (l : list string) (prf : val) :
-  (∀ `{msizeG Σ, idcntrG Σ, stateG Σ, authG Σ, seqG Σ}, ∀ vᵥ vᵢ, A vᵥ vᵢ -∗ ⌜φ vᵥ vᵢ⌝) →
-  (∀ `{msizeG Σ, idcntrG Σ, stateG Σ, authG Σ, seqG Σ}, ⊢ REL cᵥ << cᵢ : lrel_auth_comp A) →
+  (∀ `{authG Σ, seqG Σ, poisonOSG Σ}, ∀ vᵥ vᵢ, A vᵥ vᵢ -∗ ⌜φ vᵥ vᵢ⌝) →
+  (∀ `{authG Σ, seqG Σ, poisonOSG Σ}, ⊢ REL cᵥ << cᵢ : lrel_auth_comp A) →
   is_list l prf →
   adequate hash_collision NotStuck (v_run #~ cᵥ prf) σ
     (λ vᵥ σᵥ, ∃ thpᵢ σᵢ vᵢ o,
@@ -1330,10 +1870,12 @@ Proof.
   iAssert (spec_ctx) as "#Hctx"; [by iExists _|].
   iMod na_alloc as (np) "Htok".
   set (Hseq := Build_seqG _ _ np).
+  iMod pos_alloc as (γ) "Hpos".
+  set (Hpos := PoisonOSG _ _ poisonOSG_name).
 
   wp_apply wp_fupd.
   wp_apply (wp_wand with "[-]").
-  { iPoseProof (refines_run (seqG0 := Hseq) prf with "[] []") as "Hrun".
+  { iPoseProof (refines_run (seqG0 := Hseq) (poisonOSG0 := Hpos) prf with "[] []") as "Hrun".
     - by iExists _.
     - iApply Hcomp.
     - iApply ("Hrun" $! empty_ectx with "[$Hctx $Heᵢ $Htok]"). }
@@ -1355,24 +1897,24 @@ Qed.
 
 Theorem authentikit_security_syntactic (c : expr) (σ : state) (τ : type _ ⋆) prf (l : list string) :
   EqType τ →
-  ε |ₜ ∅ ⊢ₜ c : (∀: ⋆ ⇒ ⋆; ⋆ ⇒ ⋆; ⋆ ⇒ ⋆, Authentikit_func var2 var1 var0 → var0 τ) →
+  ε |ₜ ∅ ⊢ₜ c : (∀: ⋆ ⇒ ⋆; ⋆ ⇒ ⋆, Authentikit_func var1 var0 → var0 τ) →
                 is_list l prf →
-                adequate hash_collision NotStuck (v_run #~ (c #~ #~ #~ v_Authentikit) prf) σ
+                adequate hash_collision NotStuck (v_run #~ (c #~ #~ v_Authentikit) prf) σ
                   (λ vᵥ σᵥ, ∃ thpᵢ σᵢ vᵢ o,
                       vᵥ = $o ∧
                         if o is Some wᵥ then
                           (** a valid ideal execution *)
-                          rtc erased_step ([i_run #~ (c #~ #~ #~ i_Authentikit)], σ) (of_val vᵢ :: thpᵢ, σᵢ) ∧
+                          rtc erased_step ([i_run #~ (c #~ #~ i_Authentikit)], σ) (of_val vᵢ :: thpᵢ, σᵢ) ∧
                             (** and they return the same value *)
                             wᵥ = vᵢ
                         else True).
 Proof.
   intros Hτ Htyped Hprf.
-  set Σ := (#[authΣ; na_invΣ; GFunctor msizeUR; GFunctor idcntrUR; GFunctor stateUR]).
-  eapply (authentikit_security Σ (λ _ _ _ _ _, ⟦ τ ⟧ (auth_ctx ∅))); [| |done].
-  { iIntros (???????) "Hτ". by iDestruct (eq_type_sound with "Hτ") as %->. }
+  set Σ := (#[authΣ; na_invΣ; GFunctor poisonOSR]).
+  eapply (authentikit_security Σ (λ _ _ _, ⟦ τ ⟧ (auth_ctx ∅))); [| |done].
+  { iIntros (?????) "Hτ". by iDestruct (eq_type_sound with "Hτ") as %->. }
   iIntros (?????).
-  iApply refines_instantiate.
+  iApply (refines_instantiate with "[]").
   by iApply refines_typed.
 Admitted.
 
